changement symboles

proof_Isabelle/remplacement.py
@@ -1,0 +1,20 @@
+import sys
+
+txt = ''
+with open(sys.argv[1], 'r') as f:
+	txt = f.read()
+
+insid = False
+comment = False
+for i in range(len(txt)-1, -1, -1):
+	comment = (comment or txt[i-1:i+1] == '*)') and txt[i-1:i+1] != '(*'
+	insid = insid ^ (not comment and txt[i] == '"')
+	if insid and txt[i] in '|':
+		txt = txt[:i] + '\\<or>' + txt[i+1:]
+	elif insid and txt[i] in ':' and txt[i-1] != ':' and txt[(i+1)%len(txt)] != ':':
+		txt = txt[:i] + '\\<in>' + txt[i+1:]
+	elif insid and txt[i] in '~':
+		txt = txt[:i] + '\\<not>' + txt[i+1:]
+
+with open(sys.argv[1], 'w') as f:
+	txt = f.write(txt)
