proof_Isabelle/sync-mod/GenSynchModProof.thy
@@ -5,8 +5,8 @@ begin
 lemma sending:
 assumes s:"rho r p = Active s"
   and run: "HORun (k_mod.gen_HOMachine k) rho HO" (is "HORun ?A _ _")
-shows "ALL q. HOrcvdMsgs (k_mod.gen_HOMachine k) q (HO (Suc r) q) (rho r) p
-    = (if p : HO (Suc r) q then Content s else Void)" using s
+shows "\<forall>q. HOrcvdMsgs (k_mod.gen_HOMachine k) q (HO (Suc r) q) (rho r) p
+    = (if p \<in> HO (Suc r) q then Content s else Void)" using s
 unfolding HOrcvdMsgs_def k_mod.gen_HOMachine_def k_mod.gen_sendMsg_def by simp
 
 lemma sending_rec : assumes run:"HORun (k_mod.gen_HOMachine k) rho HO" (is "HORun ?A rho HO")
@@ -14,7 +14,7 @@ lemma sending_rec : assumes run:"HORun (k_mod.gen_HOMachine k) rho HO" (is "HORu
   shows "rho r q = Active v"
 proof (cases "rho r q")
   case Asleep
-  hence "?msgs q = (if q : HO (Suc r) p then Bot else Void)" unfolding HOrcvdMsgs_def by auto
+  hence "?msgs q = (if q \<in> HO (Suc r) p then Bot else Void)" unfolding HOrcvdMsgs_def by auto
   thus "rho r q = Active v" using `?msgs q = Content v` by auto
 next
   case (Active sq)
@@ -24,16 +24,16 @@ next
 qed
 
 lemma starting: 
-assumes prev: "0 < n --> rho (n-1) p = Asleep"
+assumes prev: "0 < n \<longrightarrow> rho (n-1) p = Asleep"
   and run: "HORun (k_mod.gen_HOMachine k) rho HO" 
   and act: "rho n p = Active s"
   shows "s = k_mod.gen_initState"
 proof -
-  from act have 1: "~ always_asleep rho p"
+  from act have 1: "\<not> always_asleep rho p"
     unfolding always_asleep_def by force
   from run prev act have 2: "first_awake rho p = n"
     by (rule first_awake_HO)
-  from run have "CHOinitConfig (k_mod.gen_HOMachine k) rho (%_ _. undefined)" (is "CHOinitConfig ?A _ _")
+  from run have "CHOinitConfig (k_mod.gen_HOMachine k) rho (\<lambda>_ _. undefined)" (is "CHOinitConfig ?A _ _")
     by (simp add: HORun_def CHORun_def)
   with 1 2 act have "CinitState ?A p s undefined"
     by (auto simp: CHOinitConfig_def)
@@ -46,8 +46,8 @@ and run:"HORun (k_mod.gen_HOMachine k) rho HO" (is "HORun ?A _ _")
 and "k > 2"
 shows "k_mod.gen_nextState k p s (HOrcvdMsgs ?A p (HO (Suc r) p) (rho r)) ss" (is "k_mod.gen_nextState  _ _ _ ?msgs _")
 proof -
-    have "CHOnextConfig ?A (rho r) (HO (Suc r)) (%w. undefined) (rho (Suc r))" using run by (simp add:HORun_def CHORun_def)
-    then obtain sss where "rho (Suc r) p = Active sss & CnextState ?A p s ?msgs undefined sss" using s_def 
+    have "CHOnextConfig ?A (rho r) (HO (Suc r)) (\<lambda>w. undefined) (rho (Suc r))" using run by (simp add:HORun_def CHORun_def)
+    then obtain sss where "rho (Suc r) p = Active sss \<and> CnextState ?A p s ?msgs undefined sss" using s_def 
         unfolding CHOnextConfig_def by presburger
     hence "CnextState ?A p s ?msgs undefined ss" using ss_def by auto
     thus nxt:"k_mod.gen_nextState k p s ?msgs ss" unfolding k_mod.gen_HOMachine_def by auto
@@ -57,36 +57,36 @@ qed
 If a node p is concordant in round r+2, we can deduce several facts about the incoming neighbours of p.*)
 lemma path_conc:
 assumes "rho (Suc (Suc r)) p = Active sp"
-and "x sp mod k ~= 1"
+and "x sp mod k \<noteq> 1"
 and conc_ss:"k_mod.isConc k (HOrcvdMsgs (k_mod.gen_HOMachine k) p (HO (Suc (Suc r)) p) (rho (Suc r)))"
   (is "k_mod.isConc k ?msgs")
 and run: "HORun (k_mod.gen_HOMachine k) rho HO" 
-and loop:"ALL p r. p : HO r p"
-and "q : HO (Suc (Suc r)) p"
+and loop:"\<forall>p r. p \<in> HO r p"
+and "q \<in> HO (Suc (Suc r)) p"
 and "k > 2"
 shows "k_mod.isConc k (HOrcvdMsgs (k_mod.gen_HOMachine k) q (HO (Suc r) q) (rho r))" (is "k_mod.isConc k ?msg")
-and "k_mod.isReady (HOrcvdMsgs (k_mod.gen_HOMachine k) p (HO (Suc (Suc r)) p) (rho (Suc r))) -->
+and "k_mod.isReady (HOrcvdMsgs (k_mod.gen_HOMachine k) p (HO (Suc (Suc r)) p) (rho (Suc r))) \<longrightarrow>
      k_mod.isReady (HOrcvdMsgs (k_mod.gen_HOMachine k) q (HO (Suc r) q) (rho r))"
-and "EX s. rho (Suc r) q = Active s & (Suc (x s)) mod k = x sp mod k"
+and "\<exists>s. rho (Suc r) q = Active s \<and> (Suc (x s)) mod k = x sp mod k"
 proof -
-  have "~ rho (Suc r) p = Asleep"
+  have "\<not> rho (Suc r) p = Asleep"
   proof
     assume "rho (Suc r) p = Asleep"
     hence "sp = k_mod.gen_initState" using starting[of "Suc (Suc r)" rho p k HO sp] assms by auto
-    hence "?msgs p ~= Bot" using conc_ss unfolding k_mod.isConc_def by (metis message.distinct(1) message.distinct(5))
+    hence "?msgs p \<noteq> Bot" using conc_ss unfolding k_mod.isConc_def by (metis message.distinct(1) message.distinct(5))
     thus "False" using loop `rho (Suc r) p = Asleep` unfolding HOrcvdMsgs_def by auto
   qed
   then obtain ssp where ssp:"rho (Suc r) p = Active ssp" by (cases "rho (Suc r) p") auto
   hence trans:"k_mod.gen_nextState k p ssp ?msgs sp"
     using transition[of rho "Suc r" p ssp sp k HO] assms by auto
-  have "(EX s. rho (Suc r) q = Active s & (Suc (x s)) mod k = x sp mod k) &
-    k_mod.isConc k ?msg &
-    (k_mod.isReady ?msgs --> k_mod.isReady ?msg)"
+  have "(\<exists>s. rho (Suc r) q = Active s \<and> (Suc (x s)) mod k = x sp mod k) \<and>
+    k_mod.isConc k ?msg \<and>
+    (k_mod.isReady ?msgs \<longrightarrow> k_mod.isReady ?msg)"
   proof (cases "rho (Suc r) q")
     case Asleep
     hence "?msgs q = Bot" 
       unfolding HOrcvdMsgs_def using assms by auto
-    hence "~ k_mod.isConc k ?msgs" unfolding k_mod.isConc_def by (metis message.distinct(1) message.distinct(5))
+    hence "\<not> k_mod.isConc k ?msgs" unfolding k_mod.isConc_def by (metis message.distinct(1) message.distinct(5))
     hence "False" using assms trans k_mod.gen_nextState_def by auto
     thus ?thesis by auto
   next
@@ -96,12 +96,12 @@ proof -
     ultimately have xsq:"x sq mod k = k_mod.minMsgs ?msgs mod k"
       unfolding k_mod.isConc_def by (metis message.distinct(3) message.inject)
     moreover from trans assms k_mod.gen_nextState_def have sucx:"x sp mod k = Suc (k_mod.minMsgs ?msgs) mod k" 
-    proof (cases "k_mod.ready_level1 k ?msgs ssp | k_mod.ready_level2 k ?msgs ssp")
+    proof (cases "k_mod.ready_level1 k ?msgs ssp \<or> k_mod.ready_level2 k ?msgs ssp")
       case levlup:True
       hence "x ssp mod k = k - 1" using trans
         unfolding k_mod.gen_nextState_def k_mod.ready_level2_def k_mod.ready_level1_def k_mod.isConc_def
         apply (smt ssp conc_ss k_mod.isConc_def loop message.distinct(3) message.inject run sending) done
-      moreover have "x sp = 0 | x sp = Suc (k_mod.minMsgs ?msgs)" using levlup trans unfolding k_mod.gen_nextState_def by auto
+      moreover have "x sp = 0 \<or> x sp = Suc (k_mod.minMsgs ?msgs)" using levlup trans unfolding k_mod.gen_nextState_def by auto
       ultimately show ?thesis
         by (metis Suc_diff_1 assms(7) k_mod.ready_level1_def k_mod.ready_level2_def less_Suc_eq_0_disj
         less_imp_Suc_add levlup mod_Suc mod_mod_trivial)
@@ -109,62 +109,62 @@ proof -
       case False
       thus ?thesis using trans unfolding k_mod.gen_nextState_def by auto
     qed
-    ultimately have "EX s. rho (Suc r) q = Active s & (Suc (x s)) mod k = x sp mod k"
+    ultimately have "\<exists>s. rho (Suc r) q = Active s \<and> (Suc (x s)) mod k = x sp mod k"
       using `rho (Suc r) q = Active sq`
-      exI[of "%s. rho (Suc r) q = Active s & Suc (x s) mod k = x sp mod k" sq] by (metis mod_Suc_eq)
+      exI[of "\<lambda>s. rho (Suc r) q = Active s \<and> Suc (x s) mod k = x sp mod k" sq] by (metis mod_Suc_eq)
     moreover from coc have "conc sq" unfolding k_mod.isConc_def
       by (metis `?msgs q = Content sq` message.distinct(3) message.inject)
-    hence "rho r q ~= Asleep" using starting[of "Suc r" rho q k HO sq] run Active
+    hence "rho r q \<noteq> Asleep" using starting[of "Suc r" rho q k HO sq] run Active
       unfolding k_mod.gen_initState_def Active by auto
     then obtain ssq where "rho r q = Active ssq" by (cases "rho r q") auto
     hence transq:"k_mod.gen_nextState k q ssq ?msg sq"
       using Active transition[of rho r q ssq sq k HO] assms by auto
-    from sucx xsq have "x sq mod k > 0" using `x sp mod k ~= 1`
+    from sucx xsq have "x sq mod k > 0" using `x sp mod k \<noteq> 1`
       by (metis One_nat_def Suc_lessD assms(7) gr_zeroI less_numeral_extra(4) mod_Suc numeral_2_eq_2)
     hence "k_mod.isConc k ?msg" using transq `conc sq`
       unfolding k_mod.gen_nextState_def k_mod.ready_level1_def k_mod.ready_level2_def by auto
-    moreover from transq `x sq mod k > 0` have "~ (k_mod.ready_level1 k ?msg ssq | k_mod.ready_level2 k ?msg ssq)" 
+    moreover from transq `x sq mod k > 0` have "\<not> (k_mod.ready_level1 k ?msg ssq \<or> k_mod.ready_level2 k ?msg ssq)" 
       unfolding k_mod.ready_level2_def k_mod.ready_level1_def k_mod.gen_nextState_def
       by (smt (z3) One_nat_def Suc_1 Suc_diff_1 Suc_lessD assms(7) mod_Suc mod_less neq0_conv)
     from this transq `x sq mod k > 0` assms k_mod.gen_nextState_def
-      have "ready sq --> k_mod.isReady ?msg" by auto 
-    hence "k_mod.isReady ?msgs --> k_mod.isReady ?msg"
+      have "ready sq \<longrightarrow> k_mod.isReady ?msg" by auto 
+    hence "k_mod.isReady ?msgs \<longrightarrow> k_mod.isReady ?msg"
       unfolding k_mod.isReady_def using `?msgs q = Content sq` by auto 
     ultimately show ?thesis using Active by auto
   qed
   thus "k_mod.isConc k ?msg"
-    and "k_mod.isReady ?msgs --> k_mod.isReady ?msg"
-    and "EX s. rho (Suc r) q = Active s & (Suc (x s)) mod k = x sp mod k" by auto
+    and "k_mod.isReady ?msgs \<longrightarrow> k_mod.isReady ?msg"
+    and "\<exists>s. rho (Suc r) q = Active s \<and> (Suc (x s)) mod k = x sp mod k" by auto
 qed
 
 lemma A1:
 assumes path:"k_mod.path HO xi p (t+i) (k-i)"
-and loop:"ALL p r. p : HO r p"
+and loop:"\<forall>p r. p \<in> HO r p"
 and run: "HORun (k_mod.gen_HOMachine k) rho HO" (is "HORun ?A _ _")
 and "rho (t+k) p = Active sp"
 and "k_mod.isConc k (HOrcvdMsgs (k_mod.gen_HOMachine k) p (HO (t+k) p) (rho (t+k-1)))" (is "k_mod.isConc k ?msgs")
 and "x sp mod k = 0"
 and "k > 2"
 and "i < k"
-shows "EX sxi. rho (t+i) xi = Active sxi & x sxi mod k = i &
-  (k_mod.isReady (HOrcvdMsgs (k_mod.gen_HOMachine k) p (HO (t+k) p) (rho (t+k-1))) --> ready sxi)"
+shows "\<exists>sxi. rho (t+i) xi = Active sxi \<and> x sxi mod k = i \<and>
+  (k_mod.isReady (HOrcvdMsgs (k_mod.gen_HOMachine k) p (HO (t+k) p) (rho (t+k-1))) \<longrightarrow> ready sxi)"
 proof -
   from path obtain seq where "seq 0 = xi" and "seq (k-i) = p" and
-    pat:"ALL j < k-i. seq j : HO (t+i+Suc j) (seq (Suc j))" unfolding k_mod.path_def by auto
-  have "ALL j < k-i. let msgs = HOrcvdMsgs ?A (seq (k-i-j)) (HO (t+k-j) (seq (k-i-j))) (rho (t+k-Suc j)) in
-      EX s. rho (t+k-j) (seq (k-i-j)) = Active s & x s mod k = (k - j) mod k & k_mod.isConc k msgs & (k_mod.isReady ?msgs --> k_mod.isReady msgs)"
-      (is "ALL j. ?recurr_path j")
+    pat:"\<forall>j < k-i. seq j \<in> HO (t+i+Suc j) (seq (Suc j))" unfolding k_mod.path_def by auto
+  have "\<forall>j < k-i. let msgs = HOrcvdMsgs ?A (seq (k-i-j)) (HO (t+k-j) (seq (k-i-j))) (rho (t+k-Suc j)) in
+      \<exists>s. rho (t+k-j) (seq (k-i-j)) = Active s \<and> x s mod k = (k - j) mod k \<and> k_mod.isConc k msgs \<and> (k_mod.isReady ?msgs \<longrightarrow> k_mod.isReady msgs)"
+      (is "\<forall>j. ?recurr_path j")
   proof
     fix j
-    let ?msg = "%j. HOrcvdMsgs ?A (seq (k-i-j)) (HO (t+k-j) (seq (k-i-j))) (rho (t+k-Suc j))"
-    show "j < k-i --> (let msgs = ?msg j in EX s. rho (t+k-j) (seq (k-i-j)) = Active s &
-      x s mod k = (k-j) mod k & k_mod.isConc k msgs & (k_mod.isReady ?msgs --> k_mod.isReady msgs))"
+    let ?msg = "\<lambda>j. HOrcvdMsgs ?A (seq (k-i-j)) (HO (t+k-j) (seq (k-i-j))) (rho (t+k-Suc j))"
+    show "j < k-i \<longrightarrow> (let msgs = ?msg j in \<exists>s. rho (t+k-j) (seq (k-i-j)) = Active s \<and>
+      x s mod k = (k-j) mod k \<and> k_mod.isConc k msgs \<and> (k_mod.isReady ?msgs \<longrightarrow> k_mod.isReady msgs))"
     proof (induction j)
       case 0
-      from assms `seq (k-i) = p` have "rho (t+k) (seq (k-i)) = Active sp &
-        x sp mod k = (k-0) mod k & k_mod.isConc k ?msgs & (k_mod.isReady ?msgs --> k_mod.isReady ?msgs)" by auto
-      thus "0 < k-i --> (let msgs = ?msg 0 in EX s. rho (t+k-0) (seq (k-i-0)) = Active s &
-        x s mod k = (k-0) mod k & k_mod.isConc k msgs & (k_mod.isReady ?msgs --> k_mod.isReady msgs))"
+      from assms `seq (k-i) = p` have "rho (t+k) (seq (k-i)) = Active sp \<and>
+        x sp mod k = (k-0) mod k \<and> k_mod.isConc k ?msgs \<and> (k_mod.isReady ?msgs \<longrightarrow> k_mod.isReady ?msgs)" by auto
+      thus "0 < k-i \<longrightarrow> (let msgs = ?msg 0 in \<exists>s. rho (t+k-0) (seq (k-i-0)) = Active s \<and>
+        x s mod k = (k-0) mod k \<and> k_mod.isConc k msgs \<and> (k_mod.isReady ?msgs \<longrightarrow> k_mod.isReady msgs))"
         using assms by (simp add:`seq (k-i) = p`)
     next
       case (Suc j)
@@ -172,14 +172,14 @@ proof -
       proof
         assume "Suc j < k-i"
         hence ineg1:"k-i-Suc j < k-i" and ineg2:"t+i+Suc(k-i-Suc j) = t+k-j" and ineg:"Suc (k-i-Suc j) = k-i-j" and
-        ineg3:"t+k >= Suc j" and ineg4:"Suc (t+k-Suc j) = t+k-j" and ineg5:"Suc (k - Suc(i+j)) = k-i-j" by auto
-        from this pat have link:"seq (k-i-Suc j) : HO (t+k-j) (seq (k-i-j))" by auto
+        ineg3:"t+k \<ge> Suc j" and ineg4:"Suc (t+k-Suc j) = t+k-j" and ineg5:"Suc (k - Suc(i+j)) = k-i-j" by auto
+        from this pat have link:"seq (k-i-Suc j) \<in> HO (t+k-j) (seq (k-i-j))" by auto
 
         from Suc.IH obtain ss where ss:"rho (t+k-j) (seq (k-i-j)) = Active ss"
-          and concss:"k_mod.isConc k (?msg j)" and modss:"x ss mod k = (k-j) mod k" and readyss:"k_mod.isReady ?msgs --> k_mod.isReady (?msg j)"
+          and concss:"k_mod.isConc k (?msg j)" and modss:"x ss mod k = (k-j) mod k" and readyss:"k_mod.isReady ?msgs \<longrightarrow> k_mod.isReady (?msg j)"
           using `Suc j < k-i` by (meson Suc_lessD)
 
-        have "x ss mod k ~= 1"
+        have "x ss mod k \<noteq> 1"
         proof
           assume "x ss mod k = 1"
           hence "j = k - 1" using `x ss mod k = (k-j) mod k`
@@ -188,36 +188,36 @@ proof -
           thus "False" using `Suc j < k - i` by auto
         qed
         from assms pat this ss concss modss readyss
-          obtain s where "rho (t+k-Suc j) (seq (k-i-Suc j)) = Active s & Suc (x s) mod k = x ss mod k"
-          and "k_mod.isReady ?msgs --> k_mod.isReady (?msg (Suc j))" and "k_mod.isConc k (?msg (Suc j))"
+          obtain s where "rho (t+k-Suc j) (seq (k-i-Suc j)) = Active s \<and> Suc (x s) mod k = x ss mod k"
+          and "k_mod.isReady ?msgs \<longrightarrow> k_mod.isReady (?msg (Suc j))" and "k_mod.isConc k (?msg (Suc j))"
             using path_conc[of rho "t+k-Suc (Suc j)" "seq (k-i-j)" ss k HO "seq (k-i-Suc j)"]
-            by (smt One_nat_def Suc_diff_Suc ineg4 `Suc j < k - i` `Suc j <= t + k` link ineg2
+            by (smt One_nat_def Suc_diff_Suc ineg4 `Suc j < k - i` `Suc j \<le> t + k` link ineg2
             diff_self_eq_0 ineg le_eq_less_or_eq less_diff_conv not_add_less2 plus_1_eq_Suc)
-        thus "let msgs = ?msg (Suc j) in EX s. rho (t+k-Suc j) (seq (k-i-Suc j)) = Active s &
-          x s mod k = (k-Suc j) mod k & k_mod.isConc k msgs & (k_mod.isReady ?msgs --> k_mod.isReady msgs)"
+        thus "let msgs = ?msg (Suc j) in \<exists>s. rho (t+k-Suc j) (seq (k-i-Suc j)) = Active s \<and>
+          x s mod k = (k-Suc j) mod k \<and> k_mod.isConc k msgs \<and> (k_mod.isReady ?msgs \<longrightarrow> k_mod.isReady msgs)"
           by (smt Suc_diff_Suc add_leD2 diff_Suc_1 diff_le_self ineg le_add_diff_inverse2 le_eq_less_or_eq
           less_Suc_eq_0_disj less_numeral_extra(3) linorder_not_less mod_Suc modss zero_less_diff)
       qed
     qed
   qed
   moreover have "k-i-(k-i-1) = 1" and "t+k-(k-i-1) = t+i+1" and "k-(k-i-1) = i+1" using `i < k` by auto
-  ultimately have seq1:"let msgs = HOrcvdMsgs ?A (seq 1) (HO (t+i+1) (seq 1)) (rho (t+i)) in EX ss. 
-      rho (t+i+1) (seq 1) = Active ss & x ss mod k = (i+1) mod k & k_mod.isConc k msgs &
-      (k_mod.isReady ?msgs --> k_mod.isReady msgs)" using `2 < k` allE[of ?recurr_path "k-i-1" "?recurr_path (k-i-1)"] by auto
+  ultimately have seq1:"let msgs = HOrcvdMsgs ?A (seq 1) (HO (t+i+1) (seq 1)) (rho (t+i)) in \<exists>ss. 
+      rho (t+i+1) (seq 1) = Active ss \<and> x ss mod k = (i+1) mod k \<and> k_mod.isConc k msgs \<and>
+      (k_mod.isReady ?msgs \<longrightarrow> k_mod.isReady msgs)" using `2 < k` allE[of ?recurr_path "k-i-1" "?recurr_path (k-i-1)"] by auto
   let ?msgxi = "HOrcvdMsgs ?A (seq 1) (HO (t+i+1) (seq 1)) (rho (t+i))"
-  have seq1link:"xi : HO (t+i+1) (seq 1)" using pat `seq 0 = xi` `i < k` by fastforce
-  from seq1 have concready:"k_mod.isConc k ?msgxi & (k_mod.isReady ?msgs --> k_mod.isReady ?msgxi)" by meson
-  have "rho (t+i) xi ~= Asleep"
+  have seq1link:"xi \<in> HO (t+i+1) (seq 1)" using pat `seq 0 = xi` `i < k` by fastforce
+  from seq1 have concready:"k_mod.isConc k ?msgxi \<and> (k_mod.isReady ?msgs \<longrightarrow> k_mod.isReady ?msgxi)" by meson
+  have "rho (t+i) xi \<noteq> Asleep"
   proof 
     assume "rho (t+i) xi = Asleep"
     hence "?msgxi xi = Bot" using seq1link unfolding HOrcvdMsgs_def by auto 
-    hence "~ k_mod.isConc k ?msgxi" unfolding k_mod.isConc_def by (metis message.distinct(1) message.distinct(5))
+    hence "\<not> k_mod.isConc k ?msgxi" unfolding k_mod.isConc_def by (metis message.distinct(1) message.distinct(5))
     thus "False" using seq1 by auto
   qed
   then obtain sxi where sxi:"rho (t+i) xi = Active sxi" by (cases "rho (t+i) xi") auto
   hence "?msgxi xi = Content sxi" using seq1link unfolding HOrcvdMsgs_def by (simp add: k_mod.gen_HOMachine_def k_mod.gen_sendMsg_def)
-  from sxi concready this have "k_mod.isReady ?msgs --> ready sxi" unfolding k_mod.isReady_def by auto
-  from concready loop have "rho (t+i) (seq 1) ~= Asleep" unfolding k_mod.isConc_def HOrcvdMsgs_def by fastforce
+  from sxi concready this have "k_mod.isReady ?msgs \<longrightarrow> ready sxi" unfolding k_mod.isReady_def by auto
+  from concready loop have "rho (t+i) (seq 1) \<noteq> Asleep" unfolding k_mod.isConc_def HOrcvdMsgs_def by fastforce
   then obtain ss1 where ss1:"rho (t+i) (seq 1) = Active ss1" by (cases "rho (t+i) (seq 1)") auto
   from seq1 obtain s1 where s1:"rho (t+i+1) (seq 1) = Active s1" and suci:"x s1 mod k = (i+1) mod k" by meson
   hence trans1:"k_mod.gen_nextState k (seq 1) ss1 ?msgxi s1" using transition assms ss1 s1 by auto
@@ -228,49 +228,49 @@ proof -
     by (metis (no_types, lifting) message.distinct(3) message.inject)
   ultimately have "x s1 mod k = Suc (x sxi) mod k" by (metis mod_Suc_eq)
   hence "x sxi mod k = i" using suci by (simp add: assms(8) mod_Suc)
-  thus "EX sxi. rho (t+i) xi = Active sxi & x sxi mod k = i & (k_mod.isReady ?msgs --> ready sxi)" using sxi `k_mod.isReady ?msgs --> ready sxi` by auto
+  thus "\<exists>sxi. rho (t+i) xi = Active sxi \<and> x sxi mod k = i \<and> (k_mod.isReady ?msgs \<longrightarrow> ready sxi)" using sxi `k_mod.isReady ?msgs \<longrightarrow> ready sxi` by auto
 qed
 
 lemma A2:
-assumes star:"ALL p n. k_mod.path HO xi p n k"
-and loop:"ALL p r. p : HO r p"
+assumes star:"\<forall>p n. k_mod.path HO xi p n k"
+and loop:"\<forall>p r. p \<in> HO r p"
 and run: "HORun (k_mod.gen_HOMachine k) rho HO" (is "HORun ?A _ _")
 and "k > 2"
 and "i < k"
 and ss:"rho i pp = Active ss"
-shows "level ss = 0 & x ss <= i & forc ss = 1" using `i < k` ss
+shows "level ss = 0 \<and> x ss \<le> i \<and> forc ss = 1" using `i < k` ss
 proof (induction i arbitrary: pp ss)
   case 0
   thus ?case using starting[of 0 rho pp k HO] assms unfolding k_mod.gen_initState_def by auto
 next
 case (Suc ii)
-  show "level ss = 0 & x ss <= Suc ii & forc ss = 1"
+  show "level ss = 0 \<and> x ss \<le> Suc ii \<and> forc ss = 1"
   proof (cases "rho ii pp")
     case Asleep
-    thus "level ss = 0 & x ss <= Suc ii & forc ss = 1" using run starting[of "Suc ii" rho pp k HO] Suc
+    thus "level ss = 0 \<and> x ss \<le> Suc ii \<and> forc ss = 1" using run starting[of "Suc ii" rho pp k HO] Suc
       unfolding k_mod.gen_initState_def by auto
   next
     case (Active sss)
     hence transp:"k_mod.gen_nextState k pp sss (HOrcvdMsgs ?A pp (HO (Suc ii) pp) (rho ii)) ss"
       (is "k_mod.gen_nextState _ _ _ ?msgp _") using assms transition Suc by auto
     from Active have "?msgp pp = Content sss" using loop sending run by presburger
-    have "k_mod.forceMsgs (?msgp pp) : k_mod.forceMsgs ` (range ?msgp)" by blast
+    have "k_mod.forceMsgs (?msgp pp) \<in> k_mod.forceMsgs ` (range ?msgp)" by blast
     moreover have "k_mod.forceMsgs (?msgp pp) = 1" using Suc.IH[of pp sss] Active `?msgp pp = Content sss` by (simp add: Suc_lessD `Suc ii < k` k_mod.forceMsgs.simps(1))
-    ultimately have "k_mod.maxForce ?msgp >= 1" unfolding k_mod.maxForce_def by simp
-    moreover have a:"ALL p s. ?msgp p = Content s --> x s <= ii & level s = 0 & forc s = 1" using Suc.IH sending_rec by (meson `Suc ii < k` lessI less_trans run)
-    hence "ALL p. k_mod.forceMsgs (?msgp p) <= 1" 
+    ultimately have "k_mod.maxForce ?msgp \<ge> 1" unfolding k_mod.maxForce_def by simp
+    moreover have a:"\<forall>p s. ?msgp p = Content s \<longrightarrow> x s \<le> ii \<and> level s = 0 \<and> forc s = 1" using Suc.IH sending_rec by (meson `Suc ii < k` lessI less_trans run)
+    hence "\<forall>p. k_mod.forceMsgs (?msgp p) \<le> 1" 
       unfolding k_mod.maxForce_def by (metis One_nat_def diff_Suc_1 diff_is_0_eq k_mod.forceMsgs.elims le_SucI le_zero_eq)
     ultimately have forc0:"k_mod.maxForce ?msgp = 1" unfolding k_mod.maxForce_def by (simp add: le_antisym) 
 
     moreover have "?msgp pp = Content sss" using Active sending run using loop by auto
-    ultimately have pp_inf:"?msgp pp = Content sss & forc sss = k_mod.maxForce ?msgp & x sss <= ii" using a by auto
-    let ?prop = "%sss pp ii. ?msgp pp = Content sss & forc sss = k_mod.maxForce ?msgp & x sss = ii"
-    from pp_inf have "?prop sss pp (x sss)" and "x sss <= ii" by auto
-    from pp_inf have "(LEAST i. EX s p. ?prop s p i) <= x sss" using Least_le by (smt (verit, del_insts))
-    hence "k_mod.minMsgs ?msgp <= ii" using `x sss <= ii` unfolding k_mod.minMsgs_def by auto
-    moreover from this `Suc ii < k` Active have non_levelup:"~ (k_mod.ready_level1 k ?msgp sss | k_mod.ready_level2 k ?msgp sss)"
+    ultimately have pp_inf:"?msgp pp = Content sss \<and> forc sss = k_mod.maxForce ?msgp \<and> x sss \<le> ii" using a by auto
+    let ?prop = "\<lambda>sss pp ii. ?msgp pp = Content sss \<and> forc sss = k_mod.maxForce ?msgp \<and> x sss = ii"
+    from pp_inf have "?prop sss pp (x sss)" and "x sss \<le> ii" by auto
+    from pp_inf have "(LEAST i. \<exists>s p. ?prop s p i) \<le> x sss" using Least_le by (smt (verit, del_insts))
+    hence "k_mod.minMsgs ?msgp \<le> ii" using `x sss \<le> ii` unfolding k_mod.minMsgs_def by auto
+    moreover from this `Suc ii < k` Active have non_levelup:"\<not> (k_mod.ready_level1 k ?msgp sss \<or> k_mod.ready_level2 k ?msgp sss)"
       unfolding k_mod.ready_level2_def k_mod.ready_level1_def by auto
-    ultimately have "x ss <= Suc ii" using transp unfolding k_mod.gen_nextState_def by auto
+    ultimately have "x ss \<le> Suc ii" using transp unfolding k_mod.gen_nextState_def by auto
     moreover from Suc.IH have "level ss = 0" using transp `Suc ii < k` Active unfolding k_mod.gen_nextState_def by (metis non_levelup a pp_inf)
     moreover from forc0 have "forc ss = 1" using non_levelup transp unfolding k_mod.gen_nextState_def by auto
     ultimately show ?thesis by auto
@@ -278,11 +278,11 @@ case (Suc ii)
 qed
 
 lemma A2_bis:
-assumes loop:"ALL p r. p : HO r p"
+assumes loop:"\<forall>p r. p \<in> HO r p"
 and run: "HORun (k_mod.gen_HOMachine k) rho HO" (is "HORun ?A _ _")
 and "k > 2"
 and "rho r p = Active s"
-shows "forc s >= 1 & level s <= 2" using `rho r p = Active s`
+shows "forc s \<ge> 1 \<and> level s \<le> 2" using `rho r p = Active s`
 proof (induction r arbitrary: p s)
   case 0
   thus ?case using starting[of 0 rho p k HO s] assms unfolding k_mod.gen_initState_def by auto
@@ -291,25 +291,25 @@ case (Suc rr)
   show ?case
   proof (cases "rho rr p")
     case Asleep
-    thus "forc s >= 1 & level s <= 2" using starting[of "Suc rr" rho p k HO s] Suc assms unfolding k_mod.gen_initState_def by auto
+    thus "forc s \<ge> 1 \<and> level s \<le> 2" using starting[of "Suc rr" rho p k HO s] Suc assms unfolding k_mod.gen_initState_def by auto
   next
     case (Active ss)
     let ?msgp = "HOrcvdMsgs ?A p (HO (Suc rr) p) (rho rr)"
     have "?msgp p = Content ss" using Active loop sending run by presburger
-    have "k_mod.forceMsgs (?msgp p) : k_mod.forceMsgs ` (range ?msgp)" by blast
-    moreover have "k_mod.forceMsgs (?msgp p) >= 1" using Suc.IH[of p ss] Active `?msgp p = Content ss` by (simp add: k_mod.forceMsgs.simps(1))
-    ultimately have "k_mod.maxForce ?msgp >= 1" unfolding k_mod.maxForce_def by (meson Max_ge_iff UNIV_not_empty finite finite_imageI image_is_empty)
+    have "k_mod.forceMsgs (?msgp p) \<in> k_mod.forceMsgs ` (range ?msgp)" by blast
+    moreover have "k_mod.forceMsgs (?msgp p) \<ge> 1" using Suc.IH[of p ss] Active `?msgp p = Content ss` by (simp add: k_mod.forceMsgs.simps(1))
+    ultimately have "k_mod.maxForce ?msgp \<ge> 1" unfolding k_mod.maxForce_def by (meson Max_ge_iff UNIV_not_empty finite finite_imageI image_is_empty)
     moreover have transp:"k_mod.gen_nextState k p ss ?msgp s" using Active assms transition Suc by auto
-    hence "forc s >= k_mod.maxForce ?msgp" unfolding k_mod.gen_nextState_def by auto
-    ultimately show "forc s >= 1 & level s <= 2" using transp Suc.IH[of p ss] Active unfolding k_mod.gen_nextState_def by auto
+    hence "forc s \<ge> k_mod.maxForce ?msgp" unfolding k_mod.gen_nextState_def by auto
+    ultimately show "forc s \<ge> 1 \<and> level s \<le> 2" using transp Suc.IH[of p ss] Active unfolding k_mod.gen_nextState_def by auto
   qed
 qed
 
 
 
 lemma A3:
-assumes star:"ALL p n. k_mod.path HO xi p n k"
-and loop:"ALL p r. p : HO r p"
+assumes star:"\<forall>p n. k_mod.path HO xi p n k"
+and loop:"\<forall>p r. p \<in> HO r p"
 and run: "HORun (k_mod.gen_HOMachine k) rho HO" (is "HORun ?A _ _")
 and "k > 2"
 and "rho r xi = Active sp"
@@ -320,14 +320,14 @@ and "rho (r+i) q = Active sq"
 and "rho (r+Suc i) q = Active ssq"
 and "level sq  < level ssq"
 and "i > 0"
-shows "i >= k"
+shows "i \<ge> k"
 proof (rule ccontr)
-  assume "~ i >= k"
+  assume "\<not> i \<ge> k"
   have transp:"k_mod.gen_nextState k xi sp (HOrcvdMsgs ?A xi (HO (Suc r) xi) (rho r)) ssp"
     (is "k_mod.gen_nextState _ _ _ ?msgp _") using assms transition by auto
-  have "Suc r >= k"
+  have "Suc r \<ge> k"
   proof (rule ccontr)
-    assume "~ Suc r >= k"
+    assume "\<not> Suc r \<ge> k"
     thus "False" using assms A2 by (metis not_le zero_neq_one)
   qed
   hence lev1p:"k_mod.ready_level1 k ?msgp sp" using assms transp
@@ -337,87 +337,87 @@ proof (rule ccontr)
   from transp lev1p have "x ssp mod k = 0"
     unfolding k_mod.gen_nextState_def k_mod.ready_level1_def 
     by (metis (no_types, hide_lams) Suc_diff_1 add.right_neutral assms(4) bits_mod_0 gr_implies_not_zero linorder_neqE_nat mod_Suc_eq mod_add_self1) 
-  hence val_xi:"EX sxi. rho (Suc r+i-k) xi = Active sxi & x sxi mod k = i"
-    using A1[of HO xi xi "Suc r-k" i k rho ssp] assms `Suc r >= k` `k_mod.isConc k ?msgp` `~ i >= k` self_path by auto
+  hence val_xi:"\<exists>sxi. rho (Suc r+i-k) xi = Active sxi \<and> x sxi mod k = i"
+    using A1[of HO xi xi "Suc r-k" i k rho ssp] assms `Suc r \<ge> k` `k_mod.isConc k ?msgp` `~ i \<ge> k` self_path by auto
   have transq:"k_mod.gen_nextState k q sq (HOrcvdMsgs ?A q (HO (Suc r+i) q) (rho (r+i))) ssq"
     (is "k_mod.gen_nextState _ _ _ ?msgq _") using assms transition by auto
-  hence lev1q:"k_mod.ready_level1 k ?msgq sq | k_mod.ready_level2 k ?msgq sq" using assms transp
+  hence lev1q:"k_mod.ready_level1 k ?msgq sq \<or> k_mod.ready_level2 k ?msgq sq" using assms transp
     unfolding k_mod.gen_nextState_def k_mod.ready_level1_def k_mod.ready_level2_def zero_neq_one by auto 
   hence "k_mod.isConc k ?msgq" unfolding k_mod.ready_level1_def k_mod.ready_level2_def by auto
   from transq lev1q have "x ssq mod k = 0"
     unfolding k_mod.gen_nextState_def k_mod.ready_level1_def k_mod.ready_level2_def
     by (smt (verit, best) Suc_1 Suc_diff_1 Suc_less_eq2 assms(4) less_Suc_eq_0_disj mod_Suc mod_less) 
-  hence "EX sxi. rho (Suc r+i-k) xi = Active sxi & x sxi mod k = 0" using A1[of HO xi q "Suc r-k+i" 0 k rho ssq] assms `Suc r >= k` `k_mod.isConc k ?msgq` by auto
-  thus "False" using val_xi `~ i >= k` `i > 0` by auto
+  hence "\<exists>sxi. rho (Suc r+i-k) xi = Active sxi \<and> x sxi mod k = 0" using A1[of HO xi q "Suc r-k+i" 0 k rho ssq] assms `Suc r \<ge> k` `k_mod.isConc k ?msgq` by auto
+  thus "False" using val_xi `~ i \<ge> k` `i > 0` by auto
 qed
 
 definition active_path where 
-"active_path rho HO p q n D == EX seq. seq 0 = p & seq D = q &
-    (ALL i < D. rho (n+i) (seq (Suc i)) ~= Asleep & seq i : HO (n+Suc i) (seq (Suc i)))"
+"active_path rho HO p q n D \<equiv> \<exists>seq. seq 0 = p \<and> seq D = q \<and>
+    (\<forall>i < D. rho (n+i) (seq (Suc i)) \<noteq> Asleep \<and> seq i \<in> HO (n+Suc i) (seq (Suc i)))"
 
 lemma increasing_force:
-assumes star:"ALL p n. k_mod.path HO xi p n k"
-and loop:"ALL p r. p : HO r p"
+assumes star:"\<forall>p n. k_mod.path HO xi p n k"
+and loop:"\<forall>p r. p \<in> HO r p"
 and run: "HORun (k_mod.gen_HOMachine k) rho HO" (is "HORun ?A _ _")
 and "k > 2"
 and sp:"rho t p = Active sp"
-shows "active_path rho HO p q t r --> rho (t+r) q = Active sq --> forc sp <= forc sq"
+shows "active_path rho HO p q t r \<longrightarrow> rho (t+r) q = Active sq \<longrightarrow> forc sp \<le> forc sq"
 proof (induction r arbitrary:sq q)
   case 0
-  show "active_path rho HO p q t 0 --> rho (t+0) q = Active sq --> forc sp <= forc sq" using sp unfolding active_path_def by fastforce
+  show "active_path rho HO p q t 0 \<longrightarrow> rho (t+0) q = Active sq \<longrightarrow> forc sp \<le> forc sq" using sp unfolding active_path_def by fastforce
 next
   case (Suc rr)
-  show "active_path rho HO p q t (Suc rr) --> rho (t+Suc rr) q = Active sq --> forc sp <= forc sq"
+  show "active_path rho HO p q t (Suc rr) \<longrightarrow> rho (t+Suc rr) q = Active sq \<longrightarrow> forc sp \<le> forc sq"
   proof (rule impI)+
     assume "active_path rho HO p q t (Suc rr)" and sq:"rho (t+Suc rr) q = Active sq"
-    then obtain seq where seq0:"seq 0 = p" and "seq (Suc rr) = q" and seqSuc:"ALL j < Suc rr. rho (t+j) (seq (Suc j)) ~= Asleep & seq j : HO (t+Suc j) (seq (Suc j))"
+    then obtain seq where seq0:"seq 0 = p" and "seq (Suc rr) = q" and seqSuc:"\<forall>j < Suc rr. rho (t+j) (seq (Suc j)) \<noteq> Asleep \<and> seq j \<in> HO (t+Suc j) (seq (Suc j))"
       unfolding active_path_def by auto
-    have "rho (t+rr) (seq rr) ~= Asleep"
+    have "rho (t+rr) (seq rr) \<noteq> Asleep"
     proof (cases "rr")
       case 0
-      thus "rho (t+rr) (seq rr) ~= Asleep" using seq0 sp by auto
+      thus "rho (t+rr) (seq rr) \<noteq> Asleep" using seq0 sp by auto
     next
       case (Suc rrr)
-      hence "rho (t+rr-1) (seq rr) ~= Asleep" using `seq (Suc rr) = q` seqSuc by auto
-      thus "rho (t+rr) (seq rr) ~= Asleep" using run nonAsleepAgain
+      hence "rho (t+rr-1) (seq rr) \<noteq> Asleep" using `seq (Suc rr) = q` seqSuc by auto
+      thus "rho (t+rr) (seq rr) \<noteq> Asleep" using run nonAsleepAgain
         unfolding HORun_def by (smt (z3) Suc add.commute add_Suc less_add_Suc2 plus_1_eq_Suc proc_state.simps(3) seqSuc)
     qed
     then obtain sqq where sqq:"rho (t+rr) (seq rr) = Active sqq" using run
       unfolding HORun_def by (cases "rho (t+rr) (seq rr)") auto
-    have "seq rr : HO (t+Suc rr) q" using seqSuc `seq (Suc rr) = q` by auto
+    have "seq rr \<in> HO (t+Suc rr) q" using seqSuc `seq (Suc rr) = q` by auto
     hence "active_path rho HO p (seq rr) t rr" using seq0 seqSuc unfolding active_path_def by auto
-    hence "forc sp <= forc sqq" using sqq Suc.IH by simp
+    hence "forc sp \<le> forc sqq" using sqq Suc.IH by simp
     have "HOrcvdMsgs ?A q (HO (t+Suc rr) q) (rho (t+rr)) (seq rr) = Content sqq" (is "?msgs (seq rr) = _")
       using sending[of rho "t+rr" "seq rr" sqq k HO] assms sqq `seq rr : HO (t+Suc rr) q` by auto
-    hence maxf:"k_mod.maxForce ?msgs >= forc sp" using `forc sp <= forc sqq` unfolding k_mod.maxForce_def
+    hence maxf:"k_mod.maxForce ?msgs \<ge> forc sp" using `forc sp \<le> forc sqq` unfolding k_mod.maxForce_def
       by (smt (verit) Max_ge_iff UNIV_I UNIV_not_empty finite finite_imageI image_eqI image_is_empty k_mod.forceMsgs.simps(1))
     from `seq (Suc rr) = q` seqSuc obtain ssq where "rho (t+rr) q = Active ssq" by (cases "rho (t+rr) q") auto
     hence "k_mod.gen_nextState k q ssq ?msgs sq" using assms sq transition[of _ "t+rr" q ssq sq] by auto
-    thus "forc sp <= forc sq" using maxf unfolding k_mod.gen_nextState_def by auto
+    thus "forc sp \<le> forc sq" using maxf unfolding k_mod.gen_nextState_def by auto
   qed
 qed
 
 lemma path_shrink:
 assumes "seq 0 = p"
 and "seq k = q"
-and "ALL j < k. seq j : HO (n+Suc j) (seq (Suc j))"
-and "i <= k"
+and "\<forall>j < k. seq j \<in> HO (n+Suc j) (seq (Suc j))"
+and "i \<le> k"
 shows "k_mod.path HO (seq i) q (n+i) (k-i)"
 proof  -
-  have "ALL j < k-i. seq (i+j) : HO (n+i+Suc j) (seq (i+Suc j))" using assms(3) 
+  have "\<forall>j < k-i. seq (i+j) \<in> HO (n+i+Suc j) (seq (i+Suc j))" using assms(3) 
       by (smt (z3) add.commute add.left_commute add_Suc_right less_diff_conv)
-  thus ?thesis using assms exI[of _ "%l. seq(i+l)"] unfolding k_mod.path_def by auto
+  thus ?thesis using assms exI[of _ "\<lambda>l. seq(i+l)"] unfolding k_mod.path_def by auto
 qed
 
 lemma A5:
-assumes star:"ALL p n. k_mod.path HO xi p n k"
-and loop:"ALL p r. p : HO r p"
+assumes star:"\<forall>p n. k_mod.path HO xi p n k"
+and loop:"\<forall>p r. p \<in> HO r p"
 and run: "HORun (k_mod.gen_HOMachine k) rho HO" (is "HORun ?A _ _")
 and "k > 2"
 and sp:"rho r p = Active sp"
 and maxf:"k_mod.maxForce (HOrcvdMsgs (k_mod.gen_HOMachine k) p (HO (Suc r) p) (rho r)) = f"
 and minc:"Suc (k_mod.minMsgs (HOrcvdMsgs (k_mod.gen_HOMachine k) p (HO (Suc r) p) (rho r))) = c" 
-shows "EX q sq sqq. rho (Suc r-c) q = Active sqq & level sqq = f-1 & (if f = 1 then c <= r --> rho (r-c) q = Asleep else rho (r-c) q = Active sq & level sq = f-2)"
+shows "\<exists>q sq sqq. rho (Suc r-c) q = Active sqq \<and> level sqq = f-1 \<and> (if f = 1 then c \<le> r \<longrightarrow> rho (r-c) q = Asleep else rho (r-c) q = Active sq \<and> level sq = f-2)"
   using minc sp maxf sp
 proof (induction c arbitrary:r p sp)
   case 0
@@ -425,20 +425,20 @@ proof (induction c arbitrary:r p sp)
 next
   case cc:(Suc cc)
   define msgp where "msgp = HOrcvdMsgs (k_mod.gen_HOMachine k) p (HO (Suc r) p) (rho r)"
-  have "p : HO (Suc r) p" using loop by auto
+  have "p \<in> HO (Suc r) p" using loop by auto
   hence "msgp p = Content sp" using sp run sending cc unfolding msgp_def by simp
-  have "forc sp >= 1" using A2_bis run cc(5) loop `2 < k` by blast
+  have "forc sp \<ge> 1" using A2_bis run cc(5) loop `2 < k` by blast
   hence "k_mod.forceMsgs (msgp p) > 0" using `msgp p = Content sp` by (simp add:k_mod.forceMsgs.simps(1))
-  moreover have "k_mod.forceMsgs (msgp p) : k_mod.forceMsgs ` range msgp" by auto
-  ultimately have "k_mod.maxForce msgp >= 1" using Max_ge[of "k_mod.forceMsgs ` range msgp" "k_mod.forceMsgs (msgp p)"]
+  moreover have "k_mod.forceMsgs (msgp p) \<in> k_mod.forceMsgs ` range msgp" by auto
+  ultimately have "k_mod.maxForce msgp \<ge> 1" using Max_ge[of "k_mod.forceMsgs ` range msgp" "k_mod.forceMsgs (msgp p)"]
     unfolding k_mod.maxForce_def by (metis One_nat_def finite finite_imageI le0 le_antisym not_le not_less_eq_eq)
-  hence "f >= 1" using cc unfolding msgp_def by auto
+  hence "f \<ge> 1" using cc unfolding msgp_def by auto
   obtain q where "k_mod.forceMsgs (msgp q) = f" using Max_in[of "k_mod.forceMsgs ` range msgp"] cc unfolding k_mod.maxForce_def msgp_def by auto
-  from this obtain sq where "msgp q = Content sq" using `f >= 1` by (metis One_nat_def k_mod.forceMsgs.elims not_less_eq_eq order_refl)
-  hence "EX vv s sq. msgp q = Content sq & forc sq = k_mod.maxForce msgp & x sq = vv"
+  from this obtain sq where "msgp q = Content sq" using `f \<ge> 1` by (metis One_nat_def k_mod.forceMsgs.elims not_less_eq_eq order_refl)
+  hence "\<exists>vv s sq. msgp q = Content sq \<and> forc sq = k_mod.maxForce msgp \<and> x sq = vv"
     using cc `k_mod.forceMsgs (msgp q) = f` unfolding msgp_def by (smt (z3) k_mod.forceMsgs.simps(1))
   from this obtain qq sqq where "msgp qq = Content sqq" and "forc sqq = k_mod.maxForce msgp" and "x sqq = cc"
-    using LeastI_ex[of "%cc. EX sqq qq. msgp qq = Content sqq & forc sqq = k_mod.maxForce msgp & x sqq = cc"] cc(2) unfolding k_mod.minMsgs_def msgp_def by auto
+    using LeastI_ex[of "\<lambda>cc. \<exists>sqq qq. msgp qq = Content sqq \<and> forc sqq = k_mod.maxForce msgp \<and> x sqq = cc"] cc(2) unfolding k_mod.minMsgs_def msgp_def by auto
   hence sqq:"rho r qq = Active sqq" using sending_rec run unfolding msgp_def by auto
   show ?case
   proof (cases r)
@@ -456,7 +456,7 @@ next
         define msgq where "msgq = HOrcvdMsgs (k_mod.gen_HOMachine k) qq (HO r qq) (rho (r-1))"
         hence transq:"k_mod.gen_nextState k qq sqqq msgq sqq" using `2 < k`
           transition[of rho "r-1" qq sqqq sqq k HO] sqq Active rr run unfolding msgq_def by auto
-        hence "k_mod.ready_level1 k msgq sqqq | k_mod.ready_level2 k msgq sqqq" and "forc sqq = Suc (level sqq)"
+        hence "k_mod.ready_level1 k msgq sqqq \<or> k_mod.ready_level2 k msgq sqqq" and "forc sqq = Suc (level sqq)"
           using 0 `x sqq = cc` unfolding k_mod.gen_nextState_def by auto
         hence "level sqq = Suc (level sqqq)" using transq unfolding k_mod.gen_nextState_def k_mod.ready_level1_def k_mod.ready_level2_def by auto
         thus ?thesis using Active 0 sqq `forc sqq = Suc (level sqq)` 
@@ -472,8 +472,8 @@ next
       hence "x sqq = Suc (k_mod.minMsgs msgq)" using Suc `x sqq = cc` unfolding k_mod.gen_nextState_def by auto
       moreover have "forc sqq = k_mod.maxForce msgq" using transq Suc `x sqq = cc` unfolding k_mod.gen_nextState_def by auto
       hence "k_mod.maxForce msgq = f" using cc(4) `forc sqq = k_mod.maxForce msgp` unfolding msgp_def by auto
-      ultimately have postih:"EX tr srr sr. rho (Suc r - Suc cc) tr = Active sr & level sr = f - 1 &
-       (if f = 1 then cc <= r - 1 --> rho (r - Suc cc) tr = Asleep else rho (r - Suc cc) tr = Active srr & level srr = f - 2)"
+      ultimately have postih:"\<exists>tr srr sr. rho (Suc r - Suc cc) tr = Active sr \<and> level sr = f - 1 \<and>
+       (if f = 1 then cc \<le> r - 1 \<longrightarrow> rho (r - Suc cc) tr = Asleep else rho (r - Suc cc) tr = Active srr \<and> level srr = f - 2)"
         using cc.IH[of qq "r-1" sqqq] `x sqq = cc` rr sqqq unfolding msgq_def by auto
       thus ?thesis using diff_Suc_1 rr by fastforce
     qed
@@ -485,7 +485,7 @@ next
 qed
 
 lemma level_force:
-assumes loop:"ALL p r. p : HO r p"
+assumes loop:"\<forall>p r. p \<in> HO r p"
 and run: "HORun (k_mod.gen_HOMachine k) rho HO" (is "HORun ?A _ _")
 and "k > 2"
 and sp:"rho t p = Active sp"
@@ -503,29 +503,29 @@ next
     case (Active spp)
     define msgp where "msgp = HOrcvdMsgs (k_mod.gen_HOMachine k) p (HO (Suc tt) p) (rho tt)"
     hence "msgp p = Content spp" using sending assms Active by auto
-    hence "k_mod.maxForce msgp >= forc spp" unfolding k_mod.maxForce_def by (metis Max_ge finite_UNIV finite_imageI image_eqI k_mod.forceMsgs.simps(1) rangeI)
+    hence "k_mod.maxForce msgp \<ge> forc spp" unfolding k_mod.maxForce_def by (metis Max_ge finite_UNIV finite_imageI image_eqI k_mod.forceMsgs.simps(1) rangeI)
     moreover have transp:"k_mod.gen_nextState k p spp msgp sp" using Active assms Suc transition unfolding msgp_def by auto
-    ultimately have "forc sp >= forc spp | forc sp = Suc (level sp)" unfolding k_mod.gen_nextState_def by presburger
+    ultimately have "forc sp \<ge> forc spp \<or> forc sp = Suc (level sp)" unfolding k_mod.gen_nextState_def by presburger
     thus ?thesis using Suc.IH[of spp] Active transp unfolding k_mod.gen_nextState_def by auto
   qed
 qed
 
 
 lemma A6:
-assumes star:"ALL p n. k_mod.path HO xi p n k"
-and loop:"ALL p r. p : HO r p"
+assumes star:"\<forall>p n. k_mod.path HO xi p n k"
+and loop:"\<forall>p r. p \<in> HO r p"
 and run: "HORun (k_mod.gen_HOMachine k) rho HO" (is "HORun ?A _ _")
 and "k > 2"
 and sp:"rho (t+i) p = Active sp"
-and lvup:"ALL sqq. t > 0 --> rho (t-1) q = Active sqq --> level sqq < level sq"
+and lvup:"\<forall>sqq. t > 0 \<longrightarrow> rho (t-1) q = Active sqq \<longrightarrow> level sqq < level sq"
 and sq:"rho t q = Active sq"
 and path:"active_path rho HO q p t (Suc i)"
 and msgp:"msgp = HOrcvdMsgs (k_mod.gen_HOMachine k) p (HO (Suc t+i) p) (rho (t+i))"
-shows "Suc (level sq) < k_mod.maxForce msgp | (Suc (level sq) = k_mod.maxForce msgp & (k_mod.minMsgs msgp) <= i)"
+shows "Suc (level sq) < k_mod.maxForce msgp \<or> (Suc (level sq) = k_mod.maxForce msgp \<and> (k_mod.minMsgs msgp) \<le> i)"
   using path sp msgp
 proof (induction i arbitrary:p sp msgp)
   case 0
-  hence "q : HO (Suc t) p" unfolding active_path_def by auto
+  hence "q \<in> HO (Suc t) p" unfolding active_path_def by auto
   hence msgq:"msgp q = Content sq" using 0 sending run sq by auto
   thus ?case
   proof (cases "Suc (level sq) < k_mod.maxForce msgp")
@@ -533,16 +533,16 @@ proof (induction i arbitrary:p sp msgp)
     thus ?thesis by auto
   next
     case False
-    have "k_mod.maxForce msgp >= forc sq" using msgq unfolding k_mod.maxForce_def
+    have "k_mod.maxForce msgp \<ge> forc sq" using msgq unfolding k_mod.maxForce_def
       by (metis Max_ge finite_UNIV finite_imageI image_eqI k_mod.forceMsgs.simps(1) rangeI)
     hence "forc sq = k_mod.maxForce msgp" and eq:"Suc (level sq) = k_mod.maxForce msgp" and "forc sq = Suc (level sq)"
       using False level_force[of HO k rho t q sq] assms by auto
-    hence "k_mod.minMsgs msgp <= x sq" using msgq unfolding k_mod.minMsgs_def by (metis (mono_tags, lifting) Least_le)
+    hence "k_mod.minMsgs msgp \<le> x sq" using msgq unfolding k_mod.minMsgs_def by (metis (mono_tags, lifting) Least_le)
     thus ?thesis
-    proof (cases "t > 0 --> rho (t-1) q = Asleep")
+    proof (cases "t > 0 \<longrightarrow> rho (t-1) q = Asleep")
       case True
       hence "x sq = 0" using run sq starting unfolding k_mod.gen_initState_def by (metis locState.select_convs(1))
-      thus ?thesis  using eq `k_mod.minMsgs msgp <= x sq` by auto
+      thus ?thesis  using eq `k_mod.minMsgs msgp \<le> x sq` by auto
     next
       case False
       define msgq where "msgq = HOrcvdMsgs (k_mod.gen_HOMachine k) q (HO t q) (rho (t-1))"
@@ -551,24 +551,24 @@ proof (induction i arbitrary:p sp msgp)
         using assms transition[of rho "t-1" q sqq sq k HO] False Suc_diff_1 unfolding msgq_def by fastforce
       hence "level sqq < level sq"  using lvup False sqq by auto
       hence "x sq = 0" using transq `forc sq = Suc (level sq)` unfolding k_mod.gen_nextState_def by auto
-      thus ?thesis using `k_mod.minMsgs msgp <= x sq` eq by auto
+      thus ?thesis using `k_mod.minMsgs msgp \<le> x sq` eq by auto
     qed
   qed
 next
   case (Suc ii)
   from Suc(2) obtain seq where "seq 0 = q" and "seq (Suc (Suc ii)) = p" and
-    seq:"ALL j < Suc (Suc ii). rho (t+j) (seq (Suc j)) ~= Asleep & seq j : HO (t+Suc j) (seq (Suc j))"
+    seq:"\<forall>j < Suc (Suc ii). rho (t+j) (seq (Suc j)) \<noteq> Asleep \<and> seq j \<in> HO (t+Suc j) (seq (Suc j))"
     unfolding active_path_def by auto
   hence "active_path rho HO q (seq (Suc ii)) t (Suc ii)" unfolding active_path_def by auto
   define msgs where "msgs = HOrcvdMsgs (k_mod.gen_HOMachine k) (seq (Suc ii)) (HO (t+Suc ii) (seq (Suc ii))) (rho (t+ii))"
-  from seq obtain ss where ss:"rho (t+ii) (seq (Suc ii)) = Active ss" and "seq (Suc ii) : HO (t+Suc (Suc ii)) p"
+  from seq obtain ss where ss:"rho (t+ii) (seq (Suc ii)) = Active ss" and "seq (Suc ii) \<in> HO (t+Suc (Suc ii)) p"
     using `seq (Suc (Suc ii)) = p` by (cases "rho (t+ii) (seq (Suc ii))") auto
   from ss obtain sss where sss:"rho (t+Suc ii) (seq (Suc ii)) = Active sss"
     using nonAsleepAgain[of rho "t+ii" "seq (Suc ii)" _ _ _ 1] assms unfolding HORun_def by fastforce
   hence transs:"k_mod.gen_nextState k (seq (Suc ii)) ss msgs sss" using ss transition assms unfolding msgs_def by auto
-  have ih:"Suc (level sq) < k_mod.maxForce msgs | (Suc (level sq) = k_mod.maxForce msgs & k_mod.minMsgs msgs <= ii)"
+  have ih:"Suc (level sq) < k_mod.maxForce msgs \<or> (Suc (level sq) = k_mod.maxForce msgs \<and> k_mod.minMsgs msgs \<le> ii)"
     using Suc.IH ss `active_path rho HO q (seq (Suc ii)) t (Suc ii)` msgs_def by auto
-  have "k_mod.maxForce msgs <= forc sss" and "x sss <= Suc (k_mod.minMsgs msgs)" using transs unfolding k_mod.gen_nextState_def by auto
+  have "k_mod.maxForce msgs \<le> forc sss" and "x sss \<le> Suc (k_mod.minMsgs msgs)" using transs unfolding k_mod.gen_nextState_def by auto
 
 
   have send:"msgp (seq (Suc ii)) = Content sss" using `seq (Suc ii) : HO (t+Suc (Suc ii)) p` sss
@@ -579,115 +579,115 @@ next
     thus ?thesis by auto
   next
     case False
-    have "Suc (level sq) <= k_mod.maxForce msgs" using ih by auto
-    moreover have "k_mod.maxForce msgp >= forc sss" using `msgp (seq (Suc ii)) = Content sss`
+    have "Suc (level sq) \<le> k_mod.maxForce msgs" using ih by auto
+    moreover have "k_mod.maxForce msgp \<ge> forc sss" using `msgp (seq (Suc ii)) = Content sss`
       unfolding k_mod.maxForce_def by (metis Max_ge finite_UNIV finite_imageI image_eqI k_mod.forceMsgs.simps(1) rangeI)
     ultimately have "Suc (level sq) = k_mod.maxForce msgp" and "forc sss = k_mod.maxForce msgp"
-      using False `k_mod.maxForce msgs <= forc sss` send by auto
-    moreover from this have "k_mod.minMsgs msgp <= x sss" using `msgp (seq (Suc ii)) = Content sss`
+      using False `k_mod.maxForce msgs \<le> forc sss` send by auto
+    moreover from this have "k_mod.minMsgs msgp \<le> x sss" using `msgp (seq (Suc ii)) = Content sss`
       unfolding k_mod.minMsgs_def by (metis (mono_tags, lifting) Least_le)
-    ultimately show ?thesis using `x sss <= Suc (k_mod.minMsgs msgs)` `k_mod.maxForce msgs <= forc sss` ih by linarith
+    ultimately show ?thesis using `x sss \<le> Suc (k_mod.minMsgs msgs)` `k_mod.maxForce msgs \<le> forc sss` ih by linarith
   qed
 qed
 
 lemma extend_path:
-assumes star:"ALL p n. k_mod.path HO xi p n k"
-and loop:"ALL p r. p : HO r p"
+assumes star:"\<forall>p n. k_mod.path HO xi p n k"
+and loop:"\<forall>p r. p \<in> HO r p"
 and run: "HORun (k_mod.gen_HOMachine k) rho HO" (is "HORun ?A _ _")
 and "k > 2"
 and sp:"rho (t+i) p = Active sp"
 and ssp:"rho (t+Suc i) p = Active ssp"
 and "level sp < level ssp"
 and ss:"rho (Suc t) xi = Active ss"
-and "i >= k"
+and "i \<ge> k"
 shows "active_path rho HO xi p (Suc t) i"
-and "forc ss <= k_mod.maxForce (HOrcvdMsgs (k_mod.gen_HOMachine k) p (HO (t+Suc i) p) (rho (t+i)))"
+and "forc ss \<le> k_mod.maxForce (HOrcvdMsgs (k_mod.gen_HOMachine k) p (HO (t+Suc i) p) (rho (t+i)))"
 proof -
   define msgp where "msgp = HOrcvdMsgs (k_mod.gen_HOMachine k) p (HO (t+Suc i) p) (rho (t+i))"
   have transp:"k_mod.gen_nextState k p sp msgp ssp" using assms transition unfolding msgp_def by auto
-  hence lev2p:"k_mod.ready_level1 k msgp sp | k_mod.ready_level2 k msgp sp" using assms transp unfolding k_mod.gen_nextState_def by simp 
+  hence lev2p:"k_mod.ready_level1 k msgp sp \<or> k_mod.ready_level2 k msgp sp" using assms transp unfolding k_mod.gen_nextState_def by simp 
   hence "k_mod.isConc k msgp" unfolding k_mod.ready_level1_def k_mod.ready_level2_def by auto
   from star obtain seq where "seq 0 = xi" and "seq k = p" and
-    pat:"ALL j < k. seq j : HO (Suc t+i-k+Suc j) (seq (Suc j))" (is "ALL j < _. _ : ?HOseq j") unfolding k_mod.path_def by meson
-  have nopass:"ALL j < k. rho (Suc t+i-k+j) (seq (Suc j)) ~= Asleep"
+    pat:"\<forall>j < k. seq j \<in> HO (Suc t+i-k+Suc j) (seq (Suc j))" (is "\<forall>j < _. _ \<in> ?HOseq j") unfolding k_mod.path_def by meson
+  have nopass:"\<forall>j < k. rho (Suc t+i-k+j) (seq (Suc j)) \<noteq> Asleep"
   proof (rule+)
     fix j
     assume "j < k" and "rho (Suc t+i-k+j) (seq (Suc j)) = Asleep"
     show "False"
     proof (cases "Suc j = k")
       case True
-      thus "False" using `rho (t+i) p = Active sp` `rho (Suc t+i-k+j) (seq (Suc j)) = Asleep` `i >= k` `seq k = p` by fastforce
+      thus "False" using `rho (t+i) p = Active sp` `rho (Suc t+i-k+j) (seq (Suc j)) = Asleep` `i \<ge> k` `seq k = p` by fastforce
     next
       case False
       have "k_mod.path HO (seq (Suc j)) p (Suc t+i - k + Suc j) (k - Suc j)"
         using path_shrink[of seq xi k p HO "Suc t+i - k" "Suc j"] `seq k = p` `seq 0 = xi` pat `j < k` by auto
       moreover from transp lev2p have "x ssp mod k = 0" unfolding k_mod.ready_level1_def k_mod.ready_level2_def k_mod.gen_nextState_def
         by (smt (z3) One_nat_def Suc_1 Suc_diff_1 Suc_lessD assms(4) mod_Suc mod_less)
-      ultimately obtain ss where ss:"rho (Suc t+i-k+Suc j) (seq (Suc j)) = Active ss & x ss mod k = Suc j"
-        using assms `i >= k` `k_mod.isConc k msgp` A1[of HO "seq (Suc j)" p "Suc t+i-k" "Suc j" k rho ssp] `j < k` False unfolding msgp_def by auto
-      hence "ss ~= k_mod.gen_initState" using `rho (Suc t+i-k+j) (seq (Suc j)) = Asleep` starting unfolding k_mod.gen_initState_def by auto
-      thus "False" using `rho (Suc t+i-k+j) (seq (Suc j)) = Asleep` starting[of "t+i-k+j"] `i >= k` run ss
+      ultimately obtain ss where ss:"rho (Suc t+i-k+Suc j) (seq (Suc j)) = Active ss \<and> x ss mod k = Suc j"
+        using assms `i \<ge> k` `k_mod.isConc k msgp` A1[of HO "seq (Suc j)" p "Suc t+i-k" "Suc j" k rho ssp] `j < k` False unfolding msgp_def by auto
+      hence "ss \<noteq> k_mod.gen_initState" using `rho (Suc t+i-k+j) (seq (Suc j)) = Asleep` starting unfolding k_mod.gen_initState_def by auto
+      thus "False" using `rho (Suc t+i-k+j) (seq (Suc j)) = Asleep` starting[of "t+i-k+j"] `i \<ge> k` run ss
         by (metis add_Suc_right diff_Suc_1 starting)
     qed
   qed
-  hence "rho (t+i-1) (seq (k-1)) ~= Asleep" using `2 < k` `k <= i`
+  hence "rho (t+i-1) (seq (k-1)) \<noteq> Asleep" using `2 < k` `k \<le> i`
     by (smt (z3) Nat.add_diff_assoc One_nat_def Suc_1 Suc_diff_Suc Suc_lessD diff_Suc_1 group_cancel.add1 le_add1 le_add_diff_inverse2 less_eq_Suc_le plus_1_eq_Suc)
   from this obtain sm where sm:"rho (t+i) (seq (k-1)) = Active sm"
-    using nonAsleepAgain[of rho "t+i-1" "seq (k-1)" _ _ _ 1] assms `k <= i` unfolding HORun_def by fastforce
-  let ?exseq = "%l. if l <= i-k then xi else seq (l - (i-k))"
-  have extrem:"?exseq 0 = xi & ?exseq i = p" using `seq k = p` `k <= i` assms(4) by force 
-  moreover have expat:"ALL l < i. rho (Suc t+l) (?exseq (Suc l)) ~= Asleep & ?exseq l : HO (Suc (Suc t)+l) (?exseq (Suc l))"
+    using nonAsleepAgain[of rho "t+i-1" "seq (k-1)" _ _ _ 1] assms `k \<le> i` unfolding HORun_def by fastforce
+  let ?exseq = "\<lambda>l. if l \<le> i-k then xi else seq (l - (i-k))"
+  have extrem:"?exseq 0 = xi \<and> ?exseq i = p" using `seq k = p` `k \<le> i` assms(4) by force 
+  moreover have expat:"\<forall>l < i. rho (Suc t+l) (?exseq (Suc l)) \<noteq> Asleep \<and> ?exseq l \<in> HO (Suc (Suc t)+l) (?exseq (Suc l))"
   proof (rule allI impI)+
     fix l
     assume "l < i"
-    show "rho (Suc t+l) (?exseq (Suc l)) ~= Asleep & ?exseq l : HO (Suc (Suc t)+l) (?exseq (Suc l))" 
+    show "rho (Suc t+l) (?exseq (Suc l)) \<noteq> Asleep \<and> ?exseq l \<in> HO (Suc (Suc t)+l) (?exseq (Suc l))" 
     proof (cases "l < i-k")
       case True
-      hence "rho (Suc t+l) (?exseq (Suc l)) ~= Asleep" using nonAsleepAgain[of rho "Suc t" xi] run
+      hence "rho (Suc t+l) (?exseq (Suc l)) \<noteq> Asleep" using nonAsleepAgain[of rho "Suc t" xi] run
         unfolding HORun_def by (smt (verit) Suc_leI assms(8) proc_state.simps(3))
-      thus "rho (Suc t+l) (?exseq (Suc l)) ~= Asleep & ?exseq l : HO (Suc (Suc t)+l) (?exseq (Suc l))" using loop True by auto
+      thus "rho (Suc t+l) (?exseq (Suc l)) \<noteq> Asleep \<and> ?exseq l \<in> HO (Suc (Suc t)+l) (?exseq (Suc l))" using loop True by auto
     next
       case False
-      hence "l-(i-k) < k" using `i >= k` `2 < k` by (metis `l < i` diff_diff_cancel diff_le_self less_diff_iff not_le_imp_less)
-      hence "seq (l-(i-k)) : HO (Suc t+i-k+(Suc l-(i-k))) (seq (Suc l-(i-k)))" using pat False Suc_diff_le by auto
-      hence "?exseq l : HO (Suc t+Suc l) (?exseq (Suc l))"
+      hence "l-(i-k) < k" using `i \<ge> k` `2 < k` by (metis `l < i` diff_diff_cancel diff_le_self less_diff_iff not_le_imp_less)
+      hence "seq (l-(i-k)) \<in> HO (Suc t+i-k+(Suc l-(i-k))) (seq (Suc l-(i-k)))" using pat False Suc_diff_le by auto
+      hence "?exseq l \<in> HO (Suc t+Suc l) (?exseq (Suc l))"
         using pat `seq 0 = xi` `l-(i-k) < k` False
-        by (smt (z3) Nat.add_diff_assoc `i >= k`  diff_is_0_eq' group_cancel.add1 le_add_diff_inverse nat_less_le not_less_eq)
+        by (smt (z3) Nat.add_diff_assoc `i \<ge> k`  diff_is_0_eq' group_cancel.add1 le_add_diff_inverse nat_less_le not_less_eq)
 
-      moreover have "rho (Suc t+l) (?exseq (Suc l)) ~= Asleep" using `ALL j < k. rho (Suc t+i-k+j) (seq (Suc j)) ~= Asleep` False `l-(i-k) < k` `i >= k`
+      moreover have "rho (Suc t+l) (?exseq (Suc l)) \<noteq> Asleep" using `\<forall>j < k. rho (Suc t+i-k+j) (seq (Suc j)) \<noteq> Asleep` False `l-(i-k) < k` `i \<ge> k`
         by (smt (z3) Nat.add_diff_assoc Suc_eq_plus1 Suc_le_eq add.commute add.left_commute leI le_add_diff_inverse2)
-      ultimately show "rho (Suc t+l) (?exseq (Suc l)) ~= Asleep & ?exseq l : HO (Suc (Suc t)+l) (?exseq (Suc l))" by simp
+      ultimately show "rho (Suc t+l) (?exseq (Suc l)) \<noteq> Asleep \<and> ?exseq l \<in> HO (Suc (Suc t)+l) (?exseq (Suc l))" by simp
     qed
   qed
   ultimately have patt:"active_path rho HO xi p (Suc t) i" using `seq k = p`
-    exI[of "%seqq. seqq 0 = xi & seqq i = p & (ALL j < i. rho (Suc t+j) (seqq (Suc j)) ~= Asleep & seqq j : HO (Suc t+Suc j) (seqq (Suc j)))" ?exseq]
+    exI[of "\<lambda>seqq. seqq 0 = xi \<and> seqq i = p \<and> (\<forall>j < i. rho (Suc t+j) (seqq (Suc j)) \<noteq> Asleep \<and> seqq j \<in> HO (Suc t+Suc j) (seqq (Suc j)))" ?exseq]
     unfolding active_path_def by auto
-  have "ALL j < i-1. rho (Suc t+j) (?exseq (Suc j)) ~= Asleep & ?exseq j : HO (Suc t+Suc j) (?exseq (Suc j))" using expat by auto
+  have "\<forall>j < i-1. rho (Suc t+j) (?exseq (Suc j)) \<noteq> Asleep \<and> ?exseq j \<in> HO (Suc t+Suc j) (?exseq (Suc j))" using expat by auto
   hence "active_path rho HO xi (seq (k-1)) (Suc t) (i - 1)" using `seq k = p`
-    exI[of "%seqq. seqq 0 = xi & seqq (i-1) = seq (k-1) &
-    (ALL j < i-1. rho (Suc t+j) (seqq (Suc j)) ~= Asleep & seqq j : HO (Suc t+Suc j) (seqq (Suc j)))" ?exseq] extrem expat `k <= i` `seq 0 = xi`
+    exI[of "\<lambda>seqq. seqq 0 = xi \<and> seqq (i-1) = seq (k-1) \<and>
+    (\<forall>j < i-1. rho (Suc t+j) (seqq (Suc j)) \<noteq> Asleep \<and> seqq j \<in> HO (Suc t+Suc j) (seqq (Suc j)))" ?exseq] extrem expat `k \<le> i` `seq 0 = xi`
     unfolding active_path_def by auto
-  hence "forc sm >= forc ss" using increasing_force[of HO xi k rho "Suc t" xi ss "seq (k-1)" "i-1" sm] sm assms
-    by (metis Suc_diff_1 `k <= i` add_Suc_shift dual_order.strict_trans1 less_nat_zero_code neq0_conv)
-  have "seq (k-1) : HO (Suc t+i) p" using pat `seq k = p`
+  hence "forc sm \<ge> forc ss" using increasing_force[of HO xi k rho "Suc t" xi ss "seq (k-1)" "i-1" sm] sm assms
+    by (metis Suc_diff_1 `k \<le> i` add_Suc_shift dual_order.strict_trans1 less_nat_zero_code neq0_conv)
+  have "seq (k-1) \<in> HO (Suc t+i) p" using pat `seq k = p`
     by (smt (verit, del_insts) add_Suc assms(9) assms(4) diff_Suc_1 le_add_diff_inverse2 lessI less_add_Suc2 less_iff_Suc_add nat_less_le order_trans)
   hence "msgp (seq (k-1)) = Content sm" using sm sending run unfolding msgp_def by auto
-  hence "k_mod.maxForce msgp >= forc ss" using `forc sm >= forc ss`
+  hence "k_mod.maxForce msgp \<ge> forc ss" using `forc sm \<ge> forc ss`
     by (metis (mono_tags, hide_lams) Max_ge dual_order.strict_trans1 finite_UNIV
     finite_imageI image_eqI k_mod.forceMsgs.simps(1) k_mod.maxForce_def not_le rangeI)
   thus  "active_path rho HO xi p (Suc t) i"
-    and "forc ss <= k_mod.maxForce (HOrcvdMsgs (k_mod.gen_HOMachine k) p (HO (t+Suc i) p) (rho (t+i)))"
+    and "forc ss \<le> k_mod.maxForce (HOrcvdMsgs (k_mod.gen_HOMachine k) p (HO (t+Suc i) p) (rho (t+i)))"
     using patt unfolding msgp_def by auto
 qed
 
 
 lemma level_growing:
-assumes loop:"ALL p r. p : HO r p"
+assumes loop:"\<forall>p r. p \<in> HO r p"
 and run: "HORun (k_mod.gen_HOMachine k) rho HO" (is "HORun ?A _ _")
 and "k > 2"
 and s:"rho r p = Active s"
 and "rho (r+i) p = Active ss"
-shows "level s <= level ss" using `rho (r+i) p = Active ss`
+shows "level s \<le> level ss" using `rho (r+i) p = Active ss`
 proof (induction i arbitrary: ss)
   case 0
   thus ?case using starting[of 0 rho p k HO s] assms unfolding k_mod.gen_initState_def by auto
@@ -696,15 +696,15 @@ next
   obtain sss where sss:"rho (r+rr) p = Active sss" using nonAsleepAgain[of rho r p _ _ _ rr] run s unfolding HORun_def by fastforce
   let ?msgp = "HOrcvdMsgs ?A p (HO (r+Suc rr) p) (rho (r+rr))"
   have "?msgp p = Content sss" using sss loop sending[of rho "r+rr" p sss] run by simp
-  have "k_mod.forceMsgs (?msgp p) : k_mod.forceMsgs ` (range ?msgp)" by blast
+  have "k_mod.forceMsgs (?msgp p) \<in> k_mod.forceMsgs ` (range ?msgp)" by blast
   have transp:"k_mod.gen_nextState k p sss ?msgp ss" using sss assms transition Suc by auto
-  hence "level ss >= level sss" unfolding k_mod.ready_level2_def k_mod.ready_level1_def k_mod.gen_nextState_def by auto
-  thus "level s <= level ss" using Suc.IH sss by auto
+  hence "level ss \<ge> level sss" unfolding k_mod.ready_level2_def k_mod.ready_level1_def k_mod.gen_nextState_def by auto
+  thus "level s \<le> level ss" using Suc.IH sss by auto
 qed
 
 lemma A4:
-assumes star:"ALL p n. k_mod.path HO xi p n k"
-and loop:"ALL p r. p : HO r p"
+assumes star:"\<forall>p n. k_mod.path HO xi p n k"
+and loop:"\<forall>p r. p \<in> HO r p"
 and run: "HORun (k_mod.gen_HOMachine k) rho HO" (is "HORun ?A _ _")
 and "k > 2"
 and sp:"rho (t+i) p = Active sp"
@@ -717,16 +717,16 @@ and "level s = 0"
 and "level ss = 1"
 shows "i mod k = 0"
 proof (rule ccontr)
-  assume "~ i mod k = 0"
+  assume "\<not> i mod k = 0"
   have "level sp < level ssp" using assms by auto
-  let ?n = "LEAST nn. EX s. rho nn xi = Active s & level s > 0"
-  define j where "j = (LEAST jj. EX q sq ssq. rho (t+jj) q = Active sq &
-    rho (t+Suc jj) q = Active ssq & level sq < level ssq & jj mod k ~= 0)" (is "j = (LEAST jj. EX qj sj sjj. ?P jj qj sj sjj)")
-  hence "EX i q sq ssq. rho (t+ i) q = Active sq & rho (t+Suc i) q = Active ssq & level sq < level ssq & i mod k ~= 0"
+  let ?n = "LEAST nn. \<exists>s. rho nn xi = Active s \<and> level s > 0"
+  define j where "j = (LEAST jj. \<exists>q sq ssq. rho (t+jj) q = Active sq \<and>
+    rho (t+Suc jj) q = Active ssq \<and> level sq < level ssq \<and> jj mod k \<noteq> 0)" (is "j = (LEAST jj. \<exists>qj sj sjj. ?P jj qj sj sjj)")
+  hence "\<exists>i q sq ssq. rho (t+ i) q = Active sq \<and> rho (t+Suc i) q = Active ssq \<and> level sq < level ssq \<and> i mod k \<noteq> 0"
     using `~ i mod k = 0` assms(7) assms(8) sp ssp by fastforce
   from this obtain q sq ssq where sq:"rho (t+j) q = Active sq" and ssq:"rho (t+Suc j) q = Active ssq"
-    and levsq:"level sq < level ssq" and "j mod k ~= 0"
-    using LeastI_ex[of "%jj. EX qj sj sjj. ?P jj qj sj sjj"] unfolding j_def by blast
+    and levsq:"level sq < level ssq" and "j mod k \<noteq> 0"
+    using LeastI_ex[of "\<lambda>jj. \<exists>qj sj sjj. ?P jj qj sj sjj"] unfolding j_def by blast
   define msgq where "msgq = HOrcvdMsgs (k_mod.gen_HOMachine k) q (HO (t+Suc j) q) (rho (t+j))"
   hence transq:"k_mod.gen_nextState k q sq msgq ssq" using assms transition[of rho "t+j" q sq ssq k HO] 
       sq ssq unfolding msgq_def by auto
@@ -734,46 +734,46 @@ proof (rule ccontr)
   define c where "c = k_mod.minMsgs msgq"
   have "c mod k = k-1" using levsq sq ssq transq
     unfolding c_def msgq_def k_mod.gen_nextState_def k_mod.ready_level1_def k_mod.ready_level2_def by auto
-  hence "j-Suc c mod k ~= 0"
-    using `j mod k ~= 0` by (metis One_nat_def Suc_1 Suc_lessD Suc_pred assms(4) diff_zero mod_0 mod_Suc)
+  hence "j-Suc c mod k \<noteq> 0"
+    using `j mod k \<noteq> 0` by (metis One_nat_def Suc_1 Suc_lessD Suc_pred assms(4) diff_zero mod_0 mod_Suc)
 
-  have "i >= k" using assms A3[of HO xi k rho t s ss i p sp ssp] by (metis Suc_1 `i mod k ~= 0` bits_mod_0 lessI neq0_conv)
-  have "j >= k" using assms sq ssq levsq A3[of HO xi k rho t s ss j q sq ssq] by (metis `j mod k ~= 0` bits_mod_0 neq0_conv)
+  have "i \<ge> k" using assms A3[of HO xi k rho t s ss i p sp ssp] by (metis Suc_1 `i mod k \<noteq> 0` bits_mod_0 lessI neq0_conv)
+  have "j \<ge> k" using assms sq ssq levsq A3[of HO xi k rho t s ss j q sq ssq] by (metis `j mod k \<noteq> 0` bits_mod_0 neq0_conv)
 
 
 
   obtain h sh shh where shh:"rho (t+j-c) h = Active shh" and "level shh = f-1" and
-    sh_pre:"if f = 1 then Suc c <= t+j --> rho (t+j-Suc c) h = Asleep else rho (t+j-Suc c) h = Active sh & level sh = f-2"
+    sh_pre:"if f = 1 then Suc c \<le> t+j \<longrightarrow> rho (t+j-Suc c) h = Asleep else rho (t+j-Suc c) h = Active sh \<and> level sh = f-2"
     using A5[of HO xi k rho "t+j" q sq f "Suc c"] sq assms unfolding f_def c_def msgq_def by fastforce
   define msgh where "msgh = HOrcvdMsgs (k_mod.gen_HOMachine k) h (HO (t+j-c) h) (rho (t+j-Suc c))"
-  have "forc ss <= f" and "active_path rho HO xi q (Suc t) j" using extend_path[of HO xi k rho t j q sq ssq ss]
-    assms sq ssq levsq `j >= k` unfolding msgq_def f_def by auto
+  have "forc ss \<le> f" and "active_path rho HO xi q (Suc t) j" using extend_path[of HO xi k rho t j q sq ssq ss]
+    assms sq ssq levsq `j \<ge> k` unfolding msgq_def f_def by auto
   hence "1 < f" using level_force[of HO k rho "Suc t" xi ss] sq assms by auto
-  hence "t+j >= Suc c" using sh_pre
+  hence "t+j \<ge> Suc c" using sh_pre
     `level shh = f-1` by (metis (mono_tags, lifting) One_nat_def Suc_1 Suc_diff_Suc diff_is_0_eq' diff_zero nat_le_linear not_less_eq_eq proc_state.inject shh)
   hence transh:"k_mod.gen_nextState k h sh msgh shh" using assms transition[of rho "t+j-Suc c" h sh shh k HO] sh_pre
     `level shh = f-1` unfolding msgh_def by (metis Suc_diff_le `1 < f` diff_Suc_Suc less_not_refl2 shh)
-  hence "k_mod.ready_level1 k msgh sh | k_mod.ready_level2 k msgh sh" using `level shh = f-1` sh_pre `1 < f` transh
+  hence "k_mod.ready_level1 k msgh sh \<or> k_mod.ready_level2 k msgh sh" using `level shh = f-1` sh_pre `1 < f` transh
     unfolding k_mod.gen_nextState_def by auto
-  hence "k_mod.isConc k msgh" and "k_mod.minMsgs msgh mod k = k - 1" and "x shh = 0 | x shh = Suc (k_mod.minMsgs msgh)" using transh
+  hence "k_mod.isConc k msgh" and "k_mod.minMsgs msgh mod k = k - 1" and "x shh = 0 \<or> x shh = Suc (k_mod.minMsgs msgh)" using transh
     unfolding k_mod.ready_level1_def k_mod.ready_level2_def k_mod.gen_nextState_def by auto
   hence "x shh mod k = 0" by (metis assms(4) bits_mod_0 diff_Suc_1 less_iff_Suc_add mod_Suc)
   show "False"
   proof (cases "f = 2")
     case True
-    have "j-1 >= c" using A6[of HO xi k rho "Suc t" "j-1" q sq xi ss msgq] assms True
-      sq `active_path rho HO xi q (Suc t) j` `j >= k` unfolding c_def f_def msgq_def by fastforce
-    hence "?P (j-Suc c) h sh shh" using sh_pre True shh `level shh = f-1` `j-Suc c mod k ~= 0`
+    have "j-1 \<ge> c" using A6[of HO xi k rho "Suc t" "j-1" q sq xi ss msgq] assms True
+      sq `active_path rho HO xi q (Suc t) j` `j \<ge> k` unfolding c_def f_def msgq_def by fastforce
+    hence "?P (j-Suc c) h sh shh" using sh_pre True shh `level shh = f-1` `j-Suc c mod k \<noteq> 0`
       by (smt (verit, ccfv_SIG) Nat.add_diff_assoc Suc_diff_1 `1 < f` `c mod k = k - 1` `j mod k \<noteq> 0`
       add_Suc_shift assms(4) cancel_comm_monoid_add_class.diff_cancel diff_diff_left le_add_diff_inverse2
       less_numeral_extra(4) less_trans mod_Suc mod_add_left_eq neq0_conv not_less_eq_eq plus_1_eq_Suc zero_less_one)
-    hence "EX qj sj sjj. ?P (j-Suc c) qj sj sjj" by auto
-    thus "False" using Least_le[of "%jj. EX qj sj sjj. ?P jj qj sj sjj" "j-Suc c"] by (simp add: j_def)
+    hence "\<exists>qj sj sjj. ?P (j-Suc c) qj sj sjj" by auto
+    thus "False" using Least_le[of "\<lambda>jj. \<exists>qj sj sjj. ?P jj qj sj sjj" "j-Suc c"] by (simp add: j_def)
   next
     case False
-    hence "t+j-Suc c >= k" using sh_pre A2[of HO xi k rho "t+j-Suc c" h sh] run loop `2 < k` star
+    hence "t+j-Suc c \<ge> k" using sh_pre A2[of HO xi k rho "t+j-Suc c" h sh] run loop `2 < k` star
       by (metis One_nat_def Suc_1 Suc_diff_1 Suc_diff_Suc Suc_lessD `1 < f` less_numeral_extra(4) not_le_imp_less)
-    hence "EX sss. rho (t+j-c-k) xi = Active sss & (k_mod.isReady msgh --> ready sss) & x sss mod k = 0"
+    hence "\<exists>sss. rho (t+j-c-k) xi = Active sss \<and> (k_mod.isReady msgh \<longrightarrow> ready sss) \<and> x sss mod k = 0"
       using `k_mod.isConc k msgh` A1[of HO xi h "t+j-c-k" 0 k rho shh] star loop run shh `2 < k` unfolding msgh_def
       by (smt (z3) Nat.add_0_right Suc_1 Suc_diff_Suc Suc_le_lessD Suc_lessD `Suc c \<le> t + j` `x shh mod k = 0`
       add.commute add_diff_inverse_nat diff_Suc_1 diff_zero less_trans not_le)
@@ -781,36 +781,36 @@ proof (rule ccontr)
     hence "k_mod.isReady msgh" using `k_mod.ready_level1 k msgh sh | k_mod.ready_level2 k msgh sh` transh
       unfolding k_mod.gen_nextState_def k_mod.ready_level2_def by auto
     ultimately obtain sss where sss:"rho (t+j-c-k) xi = Active sss" and "x sss mod k = 0" and "ready sss" by auto
-    hence "rho (t+j-Suc c-k) xi ~= Asleep" using starting[of "t+j-c-k" rho xi k HO sss] `t+j-Suc c >= k`
+    hence "rho (t+j-Suc c-k) xi \<noteq> Asleep" using starting[of "t+j-c-k" rho xi k HO sss] `t+j-Suc c \<ge> k`
       unfolding k_mod.gen_initState_def by (metis Nat.add_0_right One_nat_def add_Suc_shift diff_diff_left locState.select_convs(3) run)
     from this obtain ssss where "rho (t+j-Suc c-k) xi = Active ssss" by (cases "rho (t+j-Suc c-k) xi") auto
     hence transx:"k_mod.gen_nextState k xi ssss (HOrcvdMsgs (k_mod.gen_HOMachine k) xi (HO (t+j-c-k) xi) (rho (t+j-Suc c-k))) sss"
       using sss assms transition[of rho "t+j-Suc c-k" xi ssss sss k HO]
-      by (metis Suc_diff_Suc Suc_diff_le Suc_le_lessD `Suc c <= t + j` `k <= t + j - Suc c`)
+      by (metis Suc_diff_Suc Suc_diff_le Suc_le_lessD `Suc c \<le> t + j` `k \<le> t + j - Suc c`)
     hence "level sss > 0" using `x sss mod k = 0` `ready sss` unfolding k_mod.gen_nextState_def by auto
-    hence "t+j-c-k >= t" using `level s = 0` level_growing[of HO k rho "t+j-c-k" xi sss _s] s sss
+    hence "t+j-c-k \<ge> t" using `level s = 0` level_growing[of HO k rho "t+j-c-k" xi sss _s] s sss
       by (metis add_diff_inverse_nat assms(4) gr_implies_not0 le_less loop run)
     hence "j-Suc c > 0" using `2 < k` Suc_le_lessD `j mod k \<noteq> 0` `k \<le> t + j - Suc c` diff_add_inverse2 diff_le_self by linarith
-    hence "?P (j-Suc c) h sh shh" using sh_pre `1 < f` shh `level shh = f-1` `j-Suc c mod k ~= 0`
+    hence "?P (j-Suc c) h sh shh" using sh_pre `1 < f` shh `level shh = f-1` `j-Suc c mod k \<noteq> 0`
       by (smt (verit, best) Nat.add_diff_assoc Suc_1 Suc_lessD `c mod k = k - 1` `j mod k \<noteq> 0` `level shh = 2`
       add_Suc_shift diff_Suc_1 diff_is_0_eq' le_add_diff_inverse2 less_iff_Suc_add less_numeral_extra(4)
       mod_Suc mod_add_left_eq nat_le_linear zero_less_diff)
-    hence "EX qj sj sjj. ?P (j-Suc c) qj sj sjj" by auto
-    thus "False" using Least_le[of "%jj. EX qj sj sjj. ?P jj qj sj sjj" "j-Suc c"] unfolding j_def by auto
+    hence "\<exists>qj sj sjj. ?P (j-Suc c) qj sj sjj" by auto
+    thus "False" using Least_le[of "\<lambda>jj. \<exists>qj sj sjj. ?P jj qj sj sjj" "j-Suc c"] unfolding j_def by auto
   qed
 qed
 
 
 lemma safety:
-assumes star:"ALL p n. k_mod.path HO xi p n k"
-and loop:"ALL p r. p : HO r p"
+assumes star:"\<forall>p n. k_mod.path HO xi p n k"
+and loop:"\<forall>p r. p \<in> HO r p"
 and run: "HORun (k_mod.gen_HOMachine k) rho HO" (is "HORun ?A _ _")
 and "k > 2"
 shows "k_mod.safety k rho"
 proof -
-  define tt where "tt = (SOME t. EX s ss. rho t xi = Active s & rho (Suc t) xi = Active ss & level s = 0 & level ss = 1)"
-    (is "tt = (SOME t. EX s ss. ?P t s ss)")
-  have "ALL p r sp ssp. rho r p = Active sp --> level sp < 2 --> rho (Suc r) p = Active ssp --> level ssp = 2 --> r mod k = tt mod k"
+  define tt where "tt = (SOME t. \<exists>s ss. rho t xi = Active s \<and> rho (Suc t) xi = Active ss \<and> level s = 0 \<and> level ss = 1)"
+    (is "tt = (SOME t. \<exists>s ss. ?P t s ss)")
+  have "\<forall>p r sp ssp. rho r p = Active sp \<longrightarrow> level sp < 2 \<longrightarrow> rho (Suc r) p = Active ssp \<longrightarrow> level ssp = 2 \<longrightarrow> r mod k = tt mod k"
   proof (rule+)
     fix p r sp ssp
     assume sp:"rho r p = Active sp" and "level sp < 2" and ssp:"rho (Suc r) p = Active ssp" and "level ssp = 2" 
@@ -821,37 +821,37 @@ proof -
       unfolding k_mod.ready_level2_def k_mod.gen_nextState_def by auto
     hence "x ssp mod k = 0" using ssp transp unfolding k_mod.ready_level2_def k_mod.gen_nextState_def
       by (metis One_nat_def Suc_diff_1 Suc_lessD `level sp < 2` assms(4) less_trans mod_Suc mod_less)
-    moreover have "r >= k" using A2[of HO xi k rho r p sp] lev2 leI assms sp unfolding k_mod.ready_level2_def by auto
+    moreover have "r \<ge> k" using A2[of HO xi k rho r p sp] lev2 leI assms sp unfolding k_mod.ready_level2_def by auto
     ultimately obtain sss where sss:"rho (Suc r-k) xi = Active sss" and "ready sss" and "x sss mod k = 0"
       using A1[of HO xi p "Suc r-k" 0 k rho ssp] star lev2 loop run ssp `2 < k` unfolding msgp_def k_mod.ready_level2_def by auto
-    hence "rho (r-k) xi ~= Asleep" using starting[of "Suc r-k" rho xi] assms `r >= k` unfolding k_mod.gen_initState_def by fastforce
+    hence "rho (r-k) xi \<noteq> Asleep" using starting[of "Suc r-k" rho xi] assms `r \<ge> k` unfolding k_mod.gen_initState_def by fastforce
     from this obtain ss where "rho (r-k) xi = Active ss" by (cases "rho (r-k) xi") auto
     hence trans:"k_mod.gen_nextState k xi ss msgs sss" using transition
-      `r >= k` assms sss Suc_diff_le unfolding msgs_def by fastforce
+      `r \<ge> k` assms sss Suc_diff_le unfolding msgs_def by fastforce
     hence "level sss > 0" using `ready sss` `x sss mod k = 0` unfolding k_mod.gen_nextState_def by auto
     thus "r mod k = tt mod k"
-    proof (cases "EX t s ss. rho t xi = Active s & rho (Suc t) xi = Active ss & level s = 0 & level ss = 1")
+    proof (cases "\<exists>t s ss. rho t xi = Active s \<and> rho (Suc t) xi = Active ss \<and> level s = 0 \<and> level ss = 1")
       case True
       obtain t sxt ssxt where "?P t sxt ssxt" using True by auto
-      from this obtain sx ssx where "?P tt sx ssx" using someI_ex[of "%t. EX s ss. ?P t s ss"] unfolding tt_def by auto
-      hence "Suc r-k >= tt" using level_growing[of HO k rho "Suc r-k" xi sss "tt-(Suc r-k)" sx] `level sss > 0`
+      from this obtain sx ssx where "?P tt sx ssx" using someI_ex[of "\<lambda>t. \<exists>s ss. ?P t s ss"] unfolding tt_def by auto
+      hence "Suc r-k \<ge> tt" using level_growing[of HO k rho "Suc r-k" xi sss "tt-(Suc r-k)" sx] `level sss > 0`
         sss `?P tt sx ssx` assms by (metis add_diff_inverse_nat le_less not_le)
       hence "(r-tt) mod k = 0" using A4[of HO xi k rho tt "r-tt" p sp ssp sx ssx] sp ssp
         `?P tt sx ssx` assms `level ssp = 2` lev2 unfolding k_mod.ready_level2_def by auto
-      thus "r mod k = tt mod k" using `Suc r-k >= tt` mod_add_left_eq[of "r-tt" k tt] 
-        by (metis Suc_1 Suc_diff_le `k <= r` add.commute add_cancel_right_left add_diff_inverse_nat assms(4)
+      thus "r mod k = tt mod k" using `Suc r-k \<ge> tt` mod_add_left_eq[of "r-tt" k tt] 
+        by (metis Suc_1 Suc_diff_le `k \<le> r` add.commute add_cancel_right_left add_diff_inverse_nat assms(4)
         diff_less dual_order.strict_trans dual_order.strict_trans1 less_trans_Suc not_le zero_less_Suc)
     next
       case False
-      define jj where "jj = (LEAST j. EX s. rho j xi = Active s & level s > 0)" (is "_ = (LEAST j. EX s. ?Q j s)")
+      define jj where "jj = (LEAST j. \<exists>s. rho j xi = Active s \<and> level s > 0)" (is "_ = (LEAST j. \<exists>s. ?Q j s)")
       have "?Q (Suc r-k) sss" using sss `level sss > 0` by auto
-      from this obtain s where s:"rho jj xi = Active s" and "level s > 0" using LeastI_ex[of "%j. EX s. ?Q j s"] unfolding jj_def by auto
-      hence "rho (jj-1) xi ~= Asleep" using starting[of jj rho xi k HO s] assms unfolding k_mod.gen_initState_def by auto
+      from this obtain s where s:"rho jj xi = Active s" and "level s > 0" using LeastI_ex[of "\<lambda>j. \<exists>s. ?Q j s"] unfolding jj_def by auto
+      hence "rho (jj-1) xi \<noteq> Asleep" using starting[of jj rho xi k HO s] assms unfolding k_mod.gen_initState_def by auto
       from this obtain sx where sx:"rho (jj-1) xi = Active sx" by (cases "rho (jj-1) xi") auto
       have "jj > 0" using starting[of jj rho xi k HO s] `level s > 0` assms s unfolding k_mod.gen_initState_def by fastforce
       hence transj:"k_mod.gen_nextState k xi sx (HOrcvdMsgs (k_mod.gen_HOMachine k) xi (HO jj xi) (rho (jj-1))) s"
         using transition s sx assms `jj > 0` by fastforce
-      have "level sx = 0" using Least_le[of "%j. EX s. ?Q j s" "jj-1"] `jj > 0` sx
+      have "level sx = 0" using Least_le[of "\<lambda>j. \<exists>s. ?Q j s" "jj-1"] `jj > 0` sx
         unfolding jj_def by (meson diff_less neq0_conv not_le zero_less_one)
       hence "level s = 1" using transj `0 < level s` unfolding k_mod.ready_level2_def k_mod.gen_nextState_def by auto
       thus "r mod k = tt mod k" using False `level sx = 0` s `jj > 0` sx by fastforce
