proof_Isabelle/sync-mod/SyncModProof.thy
@@ -2,20 +2,20 @@ theory SyncModProof
 imports "../HOModel" SyncMod
 begin
 
-definition HOMachine_to_Algorithm :: "(Proc, pstate, SendVal) HOMachine => (Proc, pstate, SendVal) CHOAlgorithm" where
+definition HOMachine_to_Algorithm :: "(Proc, pstate, SendVal) HOMachine \<Rightarrow> (Proc, pstate, SendVal) CHOAlgorithm" where
 "HOMachine_to_Algorithm mach = 
-  (| CinitState = CinitState mach, sendMsg = sendMsg mach, CnextState = CnextState mach |)"
+  \<lparr> CinitState = CinitState mach, sendMsg = sendMsg mach, CnextState = CnextState mach \<rparr>"
 
 
-definition monovalent :: "(nat => Proc => pstate proc_state) => nat => nat => bool" where
-"monovalent rho v n == ALL p ss st. rho n p = Active ss --> rho (Suc n) p = Active st --> x st = v"
+definition monovalent :: "(nat \<Rightarrow> Proc \<Rightarrow> pstate proc_state) \<Rightarrow> nat \<Rightarrow> nat \<Rightarrow> bool" where
+"monovalent rho v n \<equiv> \<forall>p ss st. rho n p = Active ss \<longrightarrow> rho (Suc n) p = Active st \<longrightarrow> x st = v"
 
 (*lemma A1 : assumes "rho r p = Active s"
 and run:"HORun (HOMachine_to_Algorithm (k_mod.SyncMod_HOMachine k)) rho HO" (is "HORun ?A _ _")
 and "x s = k-1"
 and "p : HO (Suc r) q"
-and "rho r q ~= Asleep"
-shows "ALL st. rho (Suc r) q = Active st --> x st = 0"
+and "rho r q \<noteq> Asleep"
+shows "\<forall>st. rho (Suc r) q = Active st \<longrightarrow> x st = 0"
 proof (rule+)
     fix st
     assume "rho (Suc r) q = Active st"
@@ -23,39 +23,39 @@ proof (rule+)
     proof -
         *)
 lemma starting: 
-assumes prev: "0 < n --> rho (n-1) p = Asleep"
+assumes prev: "0 < n \<longrightarrow> rho (n-1) p = Asleep"
   and run: "HORun (HOMachine_to_Algorithm (k_mod.SyncMod_HOMachine k)) rho HO" (is "HORun ?A _ _")
   and act: "rho n p = Active s"
 shows "x s = k" 
-  and "ALL q. HOrcvdMsgs ?A q (HO (Suc n) q) (rho n) p = (if p : HO (Suc n) q then Content Nope else Void)"
-  and "~ forc s"
+  and "\<forall>q. HOrcvdMsgs ?A q (HO (Suc n) q) (rho n) p = (if p \<in> HO (Suc n) q then Content Nope else Void)"
+  and "\<not> forc s"
 proof -
-  from act have 1: "~ always_asleep rho p"
+  from act have 1: "\<not> always_asleep rho p"
     unfolding always_asleep_def by force
   from run prev act have 2: "first_awake rho p = n"
     by (rule first_awake_HO)
-  from run have "CHOinitConfig ?A rho (%_ _. undefined)"
+  from run have "CHOinitConfig ?A rho (\<lambda>_ _. undefined)"
     by (simp add: HORun_def CHORun_def)
   with 1 2 act have "CinitState ?A p s undefined"
     by (auto simp: CHOinitConfig_def)
   hence 3: "k_mod.SyncMod_initState k p s"
     by (simp add:k_mod.SyncMod_HOMachine_def HOMachine_to_Algorithm_def)
-  from 3 show "x s = k" "~ forc s" 
+  from 3 show "x s = k" "\<not> forc s" 
     by (auto simp: k_mod.SyncMod_initState_def)
-  with act show "ALL q. HOrcvdMsgs ?A q (HO (Suc n) q) (rho n) p = 
-                     (if p : HO (Suc n) q then Content Nope else Void)"
+  with act show "\<forall>q. HOrcvdMsgs ?A q (HO (Suc n) q) (rho n) p = 
+                     (if p \<in> HO (Suc n) q then Content Nope else Void)"
     by (auto simp: HOMachine_to_Algorithm_def k_mod.SyncMod_HOMachine_def 
                    k_mod.SyncMod_sendMsg_def HOrcvdMsgs_def)
 qed
 
 lemma sending : assumes run:"HORun (HOMachine_to_Algorithm (k_mod.SyncMod_HOMachine k)) rho HO" (is "HORun ?A rho HO")
 assumes "(HOrcvdMsgs ?A p (HO (Suc (Suc r)) p) (rho (Suc r))) q = Content (Val v)" (is "?msgs q = _")
-shows "? s ss. rho r q = Active s & rho (Suc r) q = Active ss & x ss = v"
+shows "? s ss. rho r q = Active s \<and> rho (Suc r) q = Active ss \<and> x ss = v"
 proof (cases "rho (Suc r) q")
     case Asleep
-    hence "?msgs q = (if q : HO (Suc (Suc r)) p then Bot else Void)"
+    hence "?msgs q = (if q \<in> HO (Suc (Suc r)) p then Bot else Void)"
         using HOrcvdMsgs_def[of ?A p "HO (Suc (Suc r)) p" "rho (Suc r)"] by auto
-    thus "? s ss. rho r q = Active s & rho (Suc r) q = Active ss & x ss = v" using `?msgs q = Content (Val v)` by auto
+    thus "? s ss. rho r q = Active s \<and> rho (Suc r) q = Active ss \<and> x ss = v" using `?msgs q = Content (Val v)` by auto
 next
     case (Active sq)
     have "sendMsg ?A q p sq = Val (x sq)"
@@ -63,20 +63,20 @@ next
         by (simp add: Active HOMachine_to_Algorithm_def k_mod.SyncMod_HOMachine_def k_mod.SyncMod_sendMsg_def)
     hence "k_mod.SyncMod_sendMsg k q p sq = Val (x sq)"
         using HOMachine_to_Algorithm_def k_mod.SyncMod_HOMachine_def by 
-        (simp add: `\<And>k. k_mod.SyncMod_HOMachine k == (|CinitState = %p st crd. k_mod.SyncMod_initState k p st,
-        sendMsg = k_mod.SyncMod_sendMsg k, CnextState = %p st msgs crd. k_mod.SyncMod_nextState k p st msgs,
+        (simp add: `\<And>k. k_mod.SyncMod_HOMachine k \<equiv> \<lparr>CinitState = \<lambda>p st crd. k_mod.SyncMod_initState k p st,
+        sendMsg = k_mod.SyncMod_sendMsg k, CnextState = \<lambda>p st msgs crd. k_mod.SyncMod_nextState k p st msgs,
         HOcommPerRd = k_mod.SyncMod_commPerRd, HOcommGlobal = k_mod.SyncMod_commGlobal,
-        HOcommSchedule = k_mod.SyncMod_commSchedule|)`)
-    hence "rho r q ~= Asleep"
+        HOcommSchedule = k_mod.SyncMod_commSchedule\<rparr>`)
+    hence "rho r q \<noteq> Asleep"
         using starting[of "Suc r" rho q k HO sq] `rho (Suc r) q = Active sq`
         by (metis SendVal.distinct(1) diff_Suc_1 k_mod.SyncMod_sendMsg_def run)
     then obtain s where "rho r q = Active s" by (cases "rho r q") auto
     moreover have "?msgs q = Content (Val (x sq))"
         using HOrcvdMsgs_def[of ?A p "HO (Suc (Suc r)) p" "rho (Suc r)"] `?msgs q = Content (Val v)`
         by (simp add: Active `sendMsg (HOMachine_to_Algorithm (k_mod.SyncMod_HOMachine k)) q p sq = Val (x sq)`)
-    ultimately have "rho r q = Active s & rho (Suc r) q = Active sq & x sq = v"
+    ultimately have "rho r q = Active s \<and> rho (Suc r) q = Active sq \<and> x sq = v"
         using `rho (Suc r) q = Active sq` `?msgs q = Content (Val v)` k_mod.SyncMod_sendMsg_def[of k q p sq] by auto
-    thus "? s ss. rho r q = Active s & rho (Suc r) q = Active ss & x ss = v"  by auto
+    thus "? s ss. rho r q = Active s \<and> rho (Suc r) q = Active ss \<and> x ss = v"  by auto
 qed
 
 lemma transition : assumes s_def:"rho r p = Active s"
@@ -86,9 +86,9 @@ and "k > 2"
 shows "k_mod.SyncMod_nextState k p s (HOrcvdMsgs ?A p (HO (Suc r) p) (rho r)) ss" (is "k_mod.SyncMod_nextState  _ _ _ ?msgs _")
 and "x ss < k"
 proof -
-    have "CHOnextConfig ?A (rho r) (HO (Suc r)) (%w. undefined) (rho (Suc r))" using run by (simp add:HORun_def CHORun_def)
-    then obtain sss where "rho (Suc r) p = Active sss & CnextState ?A p s ?msgs undefined sss" 
-        using CHOnextConfig_def[of ?A "rho r" "HO (Suc r)" "%w. undefined" "rho (Suc r)"] s_def by fastforce
+    have "CHOnextConfig ?A (rho r) (HO (Suc r)) (\<lambda>w. undefined) (rho (Suc r))" using run by (simp add:HORun_def CHORun_def)
+    then obtain sss where "rho (Suc r) p = Active sss \<and> CnextState ?A p s ?msgs undefined sss" 
+        using CHOnextConfig_def[of ?A "rho r" "HO (Suc r)" "\<lambda>w. undefined" "rho (Suc r)"] s_def by fastforce
     hence "CnextState ?A p s ?msgs undefined ss" using ss_def by auto
     hence nxt:"k_mod.SyncMod_nextState k p s ?msgs ss"
         using HOMachine_to_Algorithm_def k_mod.SyncMod_HOMachine_def[of k] by (simp add:k_mod.simp_nextState)
@@ -99,12 +99,12 @@ proof -
     next
         case non_forc:False
         thus "x ss < k"
-        proof (cases "ALL q v. ?msgs q ~= Content (Val v)")
+        proof (cases "\<forall>q v. ?msgs q \<noteq> Content (Val v)")
             case True
             thus "x ss < k" using `k > 2` nxt k_mod.SyncMod_nextState_def by auto
         next
             case False
-            hence "EX q v. ?msgs q = Content (Val v) & Suc v mod k = x ss" 
+            hence "\<exists>q v. ?msgs q = Content (Val v) \<and> Suc v mod k = x ss" 
               using non_forc nxt unfolding k_mod.SyncMod_nextState_def by metis
             thus "x ss < k" using `k > 2` by (metis less_Suc_eq_0_disj less_imp_Suc_add mod_less_divisor)
         qed
@@ -112,17 +112,17 @@ proof -
     thus "k_mod.SyncMod_nextState k p s ?msgs ss" and "x ss < k" using nxt by auto
 qed
 
-lemma sending_rec : assumes "p : HO (Suc r) q"
+lemma sending_rec : assumes "p \<in> HO (Suc r) q"
 and run:"HORun (HOMachine_to_Algorithm (k_mod.SyncMod_HOMachine k)) rho HO" (is "HORun ?A _ _")
 and "rho r p = Active s"
 and "x s < k"
 shows "HOrcvdMsgs ?A q (HO (Suc r) q) (rho r) p = Content (Val (x s))"
 proof -
     have "sendMsg ?A p q s = Val (x s)" using HOMachine_to_Algorithm_def k_mod.SyncMod_HOMachine_def `x s < k`
-        by (simp add: `!!k. k_mod.SyncMod_HOMachine k ==
-        (|CinitState = %p st crd. k_mod.SyncMod_initState k p st, sendMsg = k_mod.SyncMod_sendMsg k,
-        CnextState = %p st msgs crd. k_mod.SyncMod_nextState k p st msgs, HOcommPerRd = k_mod.SyncMod_commPerRd,
-        HOcommGlobal = k_mod.SyncMod_commGlobal, HOcommSchedule = k_mod.SyncMod_commSchedule |)` k_mod.SyncMod_sendMsg_def)
+        by (simp add: `\<And>k. k_mod.SyncMod_HOMachine k \<equiv>
+        \<lparr>CinitState = \<lambda>p st crd. k_mod.SyncMod_initState k p st, sendMsg = k_mod.SyncMod_sendMsg k,
+        CnextState = \<lambda>p st msgs crd. k_mod.SyncMod_nextState k p st msgs, HOcommPerRd = k_mod.SyncMod_commPerRd,
+        HOcommGlobal = k_mod.SyncMod_commGlobal, HOcommSchedule = k_mod.SyncMod_commSchedule \<rparr>` k_mod.SyncMod_sendMsg_def)
     thus ?thesis 
         using HOrcvdMsgs_def[of _ q "HO (Suc r) p" "rho r"] assms(1) `rho r p = Active s` k_mod.xi_nek_def[of HO p]
         by (simp add:HOrcvdMsgs_def k_mod.xi_nek_def)
@@ -135,7 +135,7 @@ and "x s = k - 1"
 and "k > 2"
 shows "monovalent rho 0 r"
 proof -
-    have "ALL p ss st. rho r p = Active ss --> rho (Suc r) p = Active st --> x st = 0"
+    have "\<forall>p ss st. rho r p = Active ss \<longrightarrow> rho (Suc r) p = Active st \<longrightarrow> x st = 0"
     proof (rule+)
         fix p
         fix ss
@@ -148,7 +148,7 @@ proof -
         hence "?msgs xi = Content (Val (x s))"
             using sending_rec[of xi HO r p k rho s] assms(1) assms(3) run k_mod.xi_nek_def `x s = k - 1` `k > 2`
             by (metis SendVal.distinct(1) diff_le_self k_mod.SyncMod_sendMsg_def nat_less_le)
-        hence non_forc:"~ (k_mod.ready_force k ?msgs ss)"
+        hence non_forc:"\<not> (k_mod.ready_force k ?msgs ss)"
                 using k_mod.ready_force_def[of k ?msgs ss] `x s = k-1` by auto
         have "CnextState ?A p ss ?msgs undefined st" 
             using HORun_def CHORun_def run CHOnextConfig_def[of ?A "rho r" _ _ "rho (Suc r)"]
@@ -157,7 +157,7 @@ proof -
         hence "k_mod.SyncMod_nextState k p ss ?msgs st"
             using HOMachine_to_Algorithm_def k_mod.SyncMod_HOMachine_def[of k]
             by (simp add: k_mod.simp_nextState)
-        hence "Suc (x s) mod k >= x st" using `?msgs xi = Content (Val (x s))` 
+        hence "Suc (x s) mod k \<ge> x st" using `?msgs xi = Content (Val (x s))` 
             k_mod.SyncMod_nextState_def[of k p ss ?msgs st] non_forc by auto
         thus "x st = 0" using `x s = k - 1` `k > 2` by auto
     qed
@@ -175,11 +175,11 @@ proof (induction i)
 next
     case (Suc i)
     let "?msgs p" = "(HOrcvdMsgs ?A p (HO (Suc (r+Suc i)) p) (rho (r+Suc i)))"
-    have no_discord:"ALL p q vv. ?msgs p q = Content (Val vv) --> vv = (v+i) mod k"
+    have no_discord:"\<forall>p q vv. ?msgs p q = Content (Val vv) \<longrightarrow> vv = (v+i) mod k"
     proof (rule+)
         fix p q vv
         assume "?msgs p q = Content (Val vv)"
-        then obtain s ss where " rho (r+i) q = Active s & rho (r+Suc i) q = Active ss & x ss = vv"
+        then obtain s ss where " rho (r+i) q = Active s \<and> rho (r+Suc i) q = Active ss \<and> x ss = vv"
             using run sending[of k rho HO p "r+i" q vv] by auto
         thus "vv = (v+i) mod k"
             using Suc.IH monovalent_def[of rho "(v+i) mod k" "r+i"] by auto
@@ -190,10 +190,10 @@ next
     moreover obtain sxx where sxx:"rho (Suc (r+i)) xi = Active sxx" 
         using run HORun_def assms(3) nonAsleepAgain[of rho r xi ?A HO _ "i+1"] by fastforce
     ultimately have "x sxx = (v+i) mod k" using Suc.IH monovalent_def[of rho "(v+i) mod k" "r+i" ] by auto
-    hence "ALL p. ?msgs p xi = Content (Val ((v+i) mod k))" (is "ALL p. ?msgs p xi = _")
+    hence "\<forall>p. ?msgs p xi = Content (Val ((v+i) mod k))" (is "\<forall>p. ?msgs p xi = _")
         using sending_rec[of xi HO "r+Suc i" _ k rho sxx] assms sxx by (simp add:k_mod.xi_nek_def )
 
-    have "ALL p ss st. rho (r+Suc i) p = Active ss --> rho (Suc (r+Suc i)) p = Active st --> x st = (v + Suc i) mod k"
+    have "\<forall>p ss st. rho (r+Suc i) p = Active ss \<longrightarrow> rho (Suc (r+Suc i)) p = Active st \<longrightarrow> x st = (v + Suc i) mod k"
     proof (rule+)
         fix p ss st
         assume "rho (r+Suc i) p = Active ss" and "rho (Suc (r+Suc i)) p = Active st"
@@ -201,19 +201,19 @@ next
         show "x st = (v + Suc i) mod k"
         proof (cases "k_mod.ready_force k (?msgs p) ss")
             case True
-            hence "EX p1 p2 v1 v2. (?msgs p) p1 = Content (Val v1) & (?msgs p) p2 = Content (Val v2) & v1 ~= v2"
+            hence "\<exists>p1 p2 v1 v2. (?msgs p) p1 = Content (Val v1) \<and> (?msgs p) p2 = Content (Val v2) \<and> v1 \<noteq> v2"
                 using k_mod.ready_force_def by blast
             then obtain p1 p2 v1 v2 where "(?msgs p) p1 = Content (Val v1)" and
-                                          "(?msgs p) p2 = Content (Val v2)" and "v1 ~= v2" by auto
-            then obtain s1 s2 ss1 ss2 where "rho (r+i) p1 = Active s1" and "rho (r+Suc i) p1 = Active ss1 & x ss1 = v1" and
-                                            "rho (r+i) p2 = Active s2" and "rho (r+Suc i) p2 = Active ss2 & x ss2 = v2"
+                                          "(?msgs p) p2 = Content (Val v2)" and "v1 \<noteq> v2" by auto
+            then obtain s1 s2 ss1 ss2 where "rho (r+i) p1 = Active s1" and "rho (r+Suc i) p1 = Active ss1 \<and> x ss1 = v1" and
+                                            "rho (r+i) p2 = Active s2" and "rho (r+Suc i) p2 = Active ss2 \<and> x ss2 = v2"
                 using run sending[of k rho HO p "r+i" p1 v1] sending[of k rho HO p "r+i" p2 v2] by auto
             hence "v1 = (v+i) mod k" and "v2 = (v+i) mod k" using Suc.IH monovalent_def[of rho "(v+i) mod k" "r+i"] by auto
-            thus "x st = (v + Suc i) mod k" using `v1 ~= v2` by auto
+            thus "x st = (v + Suc i) mod k" using `v1 \<noteq> v2` by auto
         next
             case False
-            moreover from `ALL p. ?msgs p xi = Content (Val ((v+i) mod k))` have "~ (ALL q v. (?msgs p) q ~= Content (Val v))" by auto
-            ultimately have "EX q v. ?msgs p q = Content (Val v) & Suc v mod k = x st"
+            moreover from `\<forall>p. ?msgs p xi = Content (Val ((v+i) mod k))` have "\<not> (\<forall>q v. (?msgs p) q \<noteq> Content (Val v))" by auto
+            ultimately have "\<exists>q v. ?msgs p q = Content (Val v) \<and> Suc v mod k = x st"
               using `k_mod.SyncMod_nextState k p ss (?msgs p) st`
               unfolding k_mod.SyncMod_nextState_def by fastforce
             hence "Suc ((v+i) mod k) mod k = x st" using no_discord by auto
@@ -231,8 +231,8 @@ and "k > 2"
 assumes commS:"HOcommSchedule (k_mod.SyncMod_HOMachine k) (Schedule rho)"
 shows "k_mod.liveness rho"
 proof -
-    have "EX n. Schedule rho n = UNIV" using commS by (simp add:k_mod.SyncMod_HOMachine_def k_mod.SyncMod_commSchedule_def )
-    then obtain n :: nat where "ALL p. rho n p ~= Asleep"
+    have "\<exists>n. Schedule rho n = UNIV" using commS by (simp add:k_mod.SyncMod_HOMachine_def k_mod.SyncMod_commSchedule_def )
+    then obtain n :: nat where "\<forall>p. rho n p \<noteq> Asleep"
       unfolding Schedule_def by auto
 
     have "monovalent rho 0 r" using A2 assms by auto
@@ -243,29 +243,29 @@ proof -
         using A3[where ?v = 0 and ?i = "(n+1)*k-1" and ?r = r] assms 
         by (metis (no_types, lifting) add.left_neutral less_one linorder_not_less mod_mult_self1 mod_mult_self2_is_0
         no_zero_divisors not_less0 ordered_cancel_comm_monoid_diff_class.add_diff_assoc zero_eq_add_iff_both_eq_0)
-    have "ALL p. EX rf sf. rho rf p = Active sf & fire sf"
+    have "\<forall>p. \<exists>rf sf. rho rf p = Active sf \<and> fire sf"
     proof (rule allI impI)+
         fix p
         have "r + (n+1)*(k-1) = r + ((n+1)*k-1) - n" (is "_ = ?rd - n")
             using `k > 2` by (smt Groups.mult_ac(2) Nat.add_diff_assoc2 add.commute add_diff_inverse_nat diff_Suc_Suc
             less_one linorder_not_less mod_if mod_mult_self2_is_0 mult.right_neutral no_zero_divisors not_less0 plus_1_eq_Suc
             right_diff_distrib' zero_eq_add_iff_both_eq_0)
-        hence "?rd >= n" using `k > 2`
+        hence "?rd \<ge> n" using `k > 2`
             by (metis add_gr_0 add_lessD1 less_imp_le_nat mult_pos_pos one_add_one zero_less_diff zero_less_one)
         then obtain ss where "rho (Suc ?rd) p = Active ss" 
-            using run HORun_def nonAsleepAgain[of rho n p _ _ _ "Suc ?rd - n"] using `ALL p. rho n p ~= Asleep` by fastforce
+            using run HORun_def nonAsleepAgain[of rho n p _ _ _ "Suc ?rd - n"] using `\<forall>p. rho n p \<noteq> Asleep` by fastforce
         moreover from this obtain st where "rho (Suc (Suc ?rd)) p = Active st"
             using nonAsleepAgain[of rho "Suc ?rd" p _ _ _ 1] run HORun_def Suc_diff_1 by fastforce
         ultimately have nxt:"k_mod.SyncMod_nextState k p ss (HOrcvdMsgs ?A p (HO (Suc (Suc ?rd)) p) (rho (Suc ?rd))) st"
             (is "k_mod.SyncMod_nextState  _ _ _ ?msgs _")
             using transition[of rho "Suc ?rd" p ss st] run assms(5) by auto
-        have "ALL q. ?msgs q = Void | ?msgs q = Content (Val (k-1))"
+        have "\<forall>q. ?msgs q = Void \<or> ?msgs q = Content (Val (k-1))"
         proof
             fix q
             obtain sq where "rho ?rd q = Active sq"
-                using run HORun_def nonAsleepAgain[of rho n q _ _ _ "?rd - n"] using `ALL p. rho n p ~= Asleep` `?rd >= n` by fastforce
+                using run HORun_def nonAsleepAgain[of rho n q _ _ _ "?rd - n"] using `\<forall>p. rho n p \<noteq> Asleep` `?rd \<ge> n` by fastforce
             moreover obtain sqq where "rho (Suc ?rd) q = Active sqq"
-                using run HORun_def nonAsleepAgain[of rho n q _ _ _ "Suc ?rd - n"] using `ALL p. rho n p ~= Asleep` `?rd >= n` by fastforce
+                using run HORun_def nonAsleepAgain[of rho n q _ _ _ "Suc ?rd - n"] using `\<forall>p. rho n p \<noteq> Asleep` `?rd \<ge> n` by fastforce
             ultimately have "x sqq = k-1"
                 using assms monovalent_def[of rho "k-1" ?rd] monoval assms(5) by auto
 
@@ -273,48 +273,48 @@ proof -
                 using k_mod.SyncMod_sendMsg_def[of k q p sqq] `k > 2` by auto 
             hence "sendMsg ?A q p sqq = Val (k-1)"
                 using k_mod.SyncMod_HOMachine_def HOMachine_to_Algorithm_def
-                by (simp add: `\<And>k. k_mod.SyncMod_HOMachine k == (| CinitState = %p st crd. k_mod.SyncMod_initState k p st,
-                sendMsg = k_mod.SyncMod_sendMsg k, CnextState = %p st msgs crd. k_mod.SyncMod_nextState k p st msgs,
-                HOcommPerRd = k_mod.SyncMod_commPerRd, HOcommGlobal = k_mod.SyncMod_commGlobal, HOcommSchedule = k_mod.SyncMod_commSchedule |)`)
-            hence "?msgs q = (if q : HO (Suc (Suc ?rd)) p then Content (Val (k-1)) else Void)"
+                by (simp add: `\<And>k. k_mod.SyncMod_HOMachine k \<equiv> \<lparr> CinitState = \<lambda>p st crd. k_mod.SyncMod_initState k p st,
+                sendMsg = k_mod.SyncMod_sendMsg k, CnextState = \<lambda>p st msgs crd. k_mod.SyncMod_nextState k p st msgs,
+                HOcommPerRd = k_mod.SyncMod_commPerRd, HOcommGlobal = k_mod.SyncMod_commGlobal, HOcommSchedule = k_mod.SyncMod_commSchedule \<rparr>`)
+            hence "?msgs q = (if q \<in> HO (Suc (Suc ?rd)) p then Content (Val (k-1)) else Void)"
                 using HOrcvdMsgs_def[of ?A p "HO (Suc (Suc ?rd)) p" "rho (Suc ?rd)"] `rho (Suc ?rd) q = Active sqq` by auto
-            thus "?msgs q = Void | ?msgs q = Content (Val (k-1))" by auto
+            thus "?msgs q = Void \<or> ?msgs q = Content (Val (k-1))" by auto
         qed
         hence "k_mod.ready_fire k ?msgs" using k_mod.ready_fire_def[of k ?msgs] by auto
         hence "fire st" using nxt k_mod.SyncMod_nextState_def by auto
-        hence "rho (Suc (Suc ?rd)) p = Active st & fire st" using `rho (Suc (Suc ?rd)) p = Active st` by auto
-        thus "? rf sf. rho rf p = Active sf & fire sf" by auto
+        hence "rho (Suc (Suc ?rd)) p = Active st \<and> fire st" using `rho (Suc (Suc ?rd)) p = Active st` by auto
+        thus "? rf sf. rho rf p = Active sf \<and> fire sf" by auto
     qed
     thus "k_mod.liveness rho" using k_mod.liveness_def by fastforce
 qed
 
 definition round_force where
-"round_force rho p == Eps (%r. EX sa saa. rho r p = Active sa & (~ forc sa) & rho (Suc r) p = Active saa & forc saa)"
+"round_force rho p \<equiv> Eps (\<lambda>r. \<exists>sa saa. rho r p = Active sa \<and> (\<not> forc sa) \<and> rho (Suc r) p = Active saa \<and> forc saa)"
 
 lemma nonForceAgain : assumes "round_force rho p < n"
 and run:"HORun (HOMachine_to_Algorithm (k_mod.SyncMod_HOMachine k)) rho HO" (is "HORun ?A _ _")
 and "rho n p = Active sr"
 and "rho (Suc n) p = Active s"
 and "k > 2"
-shows "~ k_mod.ready_force k (HOrcvdMsgs ?A p (HO (Suc n) p) (rho n)) sr" (is "~ k_mod.ready_force k ?msgs sr")
-proof (cases "EX r sa saa. rho r p = Active sa & (~ forc sa) & rho (Suc r) p = Active saa & forc saa")
+shows "\<not> k_mod.ready_force k (HOrcvdMsgs ?A p (HO (Suc n) p) (rho n)) sr" (is "\<not> k_mod.ready_force k ?msgs sr")
+proof (cases "\<exists>r sa saa. rho r p = Active sa \<and> (\<not> forc sa) \<and> rho (Suc r) p = Active saa \<and> forc saa")
     case True
-    then obtain r where "EX sa saa. rho r p = Active sa & (~ forc sa) & rho (Suc r) p = Active saa & forc saa" by auto
-    then obtain sa saa where rd_forc:"rho (round_force rho p) p = Active sa & (~ forc sa) & rho (Suc (round_force rho p)) p = Active saa & forc saa"
-        using round_force_def[of rho p]  someI[of "%r. EX sa saa. rho r p = Active sa & (~ forc sa) & rho (Suc r) p = Active saa & forc saa" r] by auto 
-    have "ALL i ss. rho (Suc i + round_force rho p) p = Active ss --> forc ss"
+    then obtain r where "\<exists>sa saa. rho r p = Active sa \<and> (\<not> forc sa) \<and> rho (Suc r) p = Active saa \<and> forc saa" by auto
+    then obtain sa saa where rd_forc:"rho (round_force rho p) p = Active sa \<and> (\<not> forc sa) \<and> rho (Suc (round_force rho p)) p = Active saa \<and> forc saa"
+        using round_force_def[of rho p]  someI[of "\<lambda>r. \<exists>sa saa. rho r p = Active sa \<and> (\<not> forc sa) \<and> rho (Suc r) p = Active saa \<and> forc saa" r] by auto 
+    have "\<forall>i ss. rho (Suc i + round_force rho p) p = Active ss \<longrightarrow> forc ss"
     proof (rule allI)+
         fix i ss
-        show "rho (Suc i + round_force rho p) p = Active ss --> forc ss"
+        show "rho (Suc i + round_force rho p) p = Active ss \<longrightarrow> forc ss"
         proof (induction i arbitrary:ss)
             case 0
-            thus "rho (Suc 0 + round_force rho p) p = Active ss --> forc ss" using rd_forc by auto
+            thus "rho (Suc 0 + round_force rho p) p = Active ss \<longrightarrow> forc ss" using rd_forc by auto
         next
             case (Suc ii)
             moreover obtain st where "rho (Suc ii + round_force rho p) p = Active st" 
                 using nonAsleepAgain[of rho "round_force rho p" p ?A HO _ "Suc ii"] run HORun_def rd_forc by (metis add.commute proc_state.distinct(1))
             ultimately have "forc st" using add.commute[of "Suc ii" "round_force rho p"] by auto
-            show "rho (Suc (Suc ii) + round_force rho p) p = Active ss --> forc ss" 
+            show "rho (Suc (Suc ii) + round_force rho p) p = Active ss \<longrightarrow> forc ss" 
             proof
                 assume "rho (Suc (Suc ii) + round_force rho p) p = Active ss" 
                 hence "k_mod.SyncMod_nextState k p st (HOrcvdMsgs ?A p (HO (Suc (Suc ii + round_force rho p)) p) (rho (Suc ii + round_force rho p))) ss"
@@ -323,15 +323,15 @@ proof (cases "EX r sa saa. rho r p = Active sa & (~ forc sa) & rho (Suc r) p = A
             qed
         qed
     qed
-    hence "ALL s. rho n p = Active sr --> forc sr"
-        using assms(1) allE[of "%i. ALL ss. rho (Suc i + round_force rho p) p = Active ss --> forc ss" "n - Suc (round_force rho p)"] by auto
+    hence "\<forall>s. rho n p = Active sr \<longrightarrow> forc sr"
+        using assms(1) allE[of "\<lambda>i. \<forall>ss. rho (Suc i + round_force rho p) p = Active ss \<longrightarrow> forc ss" "n - Suc (round_force rho p)"] by auto
     thus ?thesis using k_mod.ready_force_def[of k ?msgs sr] by (metis assms(3))
 next
     case False
-    hence "~ forc s | forc sr" using assms(3) assms(4) by auto
+    hence "\<not> forc s \<or> forc sr" using assms(3) assms(4) by auto
     thus ?thesis
     proof
-        assume "~ forc s"
+        assume "\<not> forc s"
         have "k_mod.SyncMod_nextState k p sr ?msgs s" using transition[of rho n p sr s k HO] assms by auto
         thus ?thesis using k_mod.SyncMod_nextState_def[of k p sr _ s] by (simp add:`~ forc s` k_mod.ready_force_def)
     next
@@ -340,49 +340,49 @@ next
     qed
 qed
 
-lemma neverForce : assumes "~ (EX sa saa. rho (round_force rho xi) xi = Active sa & (~ forc sa) & rho (Suc (round_force rho xi)) xi = Active saa & forc saa)"
+lemma neverForce : assumes "\<not> (\<exists>sa saa. rho (round_force rho xi) xi = Active sa \<and> (\<not> forc sa) \<and> rho (Suc (round_force rho xi)) xi = Active saa \<and> forc saa)"
 and run:"HORun (HOMachine_to_Algorithm (k_mod.SyncMod_HOMachine k)) rho HO" (is "HORun ?A _ _")
-shows "ALL i. rho i xi = Active st --> ~ forc st"
+shows "\<forall>i. rho i xi = Active st \<longrightarrow> \<not> forc st"
 proof
     fix i
-    show "rho i xi = Active st --> ~ forc st"
+    show "rho i xi = Active st \<longrightarrow> \<not> forc st"
     proof (induction i arbitrary:st)
         case 0
-        show "rho 0 xi = Active st --> ~ forc st" using assms starting[of 0 rho xi ] by auto
+        show "rho 0 xi = Active st \<longrightarrow> \<not> forc st" using assms starting[of 0 rho xi ] by auto
     next
         case (Suc ii)
-        show "rho (Suc ii) xi = Active st --> ~ forc st"
+        show "rho (Suc ii) xi = Active st \<longrightarrow> \<not> forc st"
         proof (cases "rho ii xi")
             case Asleep
-            thus "rho (Suc ii) xi = Active st --> ~ forc st" using run starting[of "Suc ii" rho xi ] by auto
+            thus "rho (Suc ii) xi = Active st \<longrightarrow> \<not> forc st" using run starting[of "Suc ii" rho xi ] by auto
         next
             case (Active sxi)
-            moreover have "ALL sa saa l. rho l xi = Active sa --> (~ forc sa) --> rho (Suc l) xi = Active saa --> (~ forc saa)"
+            moreover have "\<forall>sa saa l. rho l xi = Active sa \<longrightarrow> (\<not> forc sa) \<longrightarrow> rho (Suc l) xi = Active saa \<longrightarrow> (\<not> forc saa)"
                 using assms(1)
-                someI_ex[of "%l. EX sa saa. rho l xi = Active sa & (~ forc sa) & rho (Suc l) xi = Active saa & forc saa"]
+                someI_ex[of "\<lambda>l. \<exists>sa saa. rho l xi = Active sa \<and> (\<not> forc sa) \<and> rho (Suc l) xi = Active saa \<and> forc saa"]
                 round_force_def by (smt Eps_cong)
-            ultimately show "rho (Suc ii) xi = Active st --> ~ forc st" using Suc.IH[of sxi] by auto
+            ultimately show "rho (Suc ii) xi = Active st \<longrightarrow> \<not> forc st" using Suc.IH[of sxi] by auto
         qed
     qed
 qed
 
 lemma A5 : assumes "k_mod.xi_nek HO xi"
 and run:"HORun (HOMachine_to_Algorithm (k_mod.SyncMod_HOMachine k)) rho HO" (is "HORun ?A _ _")
-and "rho r xi ~= Asleep"
+and "rho r xi \<noteq> Asleep"
 and "rho (Suc r) xi = Active sxi"
 and "k > 2"
 and commS:"HOcommSchedule (k_mod.SyncMod_HOMachine k) (Schedule rho)"
-and "ALL p. round_force rho p < Suc r"
+and "\<forall>p. round_force rho p < Suc r"
 and "rho (Suc r) p = Active sp"
 and "rho (Suc (Suc r)) p = Active spp"
-shows "x spp <= (Suc (x sxi)) mod k"
+shows "x spp \<le> (Suc (x sxi)) mod k"
 proof -
     from assms(3) obtain s where "rho r xi = Active s" by (cases "rho r xi") auto
     have nxt:"k_mod.SyncMod_nextState k p sp (HOrcvdMsgs ?A p (HO (Suc (Suc r)) p) (rho (Suc r))) spp" (is "k_mod.SyncMod_nextState k p sp (?msgs p) spp")
         using transition[of rho "Suc r" p sp spp k HO] assms by auto
     obtain sx where "rho (Suc r) xi = Active sx" using run HORun_def nonAsleepAgain[of rho r xi _ _ _ 1] assms(3) by fastforce
     hence "x sxi < k" and "x sx < k" using `rho r xi = Active s` transition run assms by auto
-    have "~ k_mod.ready_force k (?msgs p) sp" using nonForceAgain[of rho p "Suc r" k HO sp spp] `k > 2` assms(8) assms(9) assms(7) run less_SucI by blast
+    have "\<not> k_mod.ready_force k (?msgs p) sp" using nonForceAgain[of rho p "Suc r" k HO sp spp] `k > 2` assms(8) assms(9) assms(7) run less_SucI by blast
     moreover have "?msgs p xi = Content (Val (x sxi))"
         using sending_rec[of xi HO "Suc r" p k rho sxi] assms(1) `rho (Suc r) xi = Active sxi` run k_mod.xi_nek_def `x sxi < k` by metis
     ultimately show ?thesis using k_mod.SyncMod_nextState_def `k > 2` nxt by auto
@@ -400,10 +400,10 @@ proof -
     hence "monovalent rho (k-1) (r+(k - 1 - v mod k))"
         by (smt One_nat_def Suc_leI assms(5) diff_diff_cancel diff_is_0_eq mod_add_left_eq mod_less
         mod_less_divisor not_less ordered_cancel_comm_monoid_diff_class.add_diff_inverse plus_1_eq_Suc zero_less_Suc)
-    moreover have "rho (r+(k - 1 - v mod k)) xi ~= Asleep" using nonAsleepAgain[of rho r xi _ _ _ "k - 1 - v mod k"] assms(3) run HORun_def
+    moreover have "rho (r+(k - 1 - v mod k)) xi \<noteq> Asleep" using nonAsleepAgain[of rho r xi _ _ _ "k - 1 - v mod k"] assms(3) run HORun_def
         by (smt add.commute proc_state.distinct(1))
     then obtain sxi where sxi_def:"rho (r+(k - 1 - v mod k)) xi = Active sxi" by (cases "rho (r+(k - 1 - v mod k)) xi") auto
-    moreover from this have "rho (Suc (r+(k - 1 - v mod k))) xi ~= Asleep" using nonAsleepAgain[of rho "r+(k - 1 - v mod k)" xi _ _ _ 1] run HORun_def by fastforce
+    moreover from this have "rho (Suc (r+(k - 1 - v mod k))) xi \<noteq> Asleep" using nonAsleepAgain[of rho "r+(k - 1 - v mod k)" xi _ _ _ 1] run HORun_def by fastforce
     then obtain sxii where sxii_def:"rho (Suc (r+(k - 1 - v mod k))) xi = Active sxii" by (cases "rho (Suc (r+(k - 1 - v mod k))) xi") auto
     ultimately have "x sxii = k-1" using monovalent_def[of rho "k-1" "r+(k - 1 - v mod k)"] assms(3) by auto
     thus ?thesis using A4 assms sxi_def sxii_def by auto
@@ -417,9 +417,9 @@ and "k > 2"
 and "round_force rho xi < r"
 shows "x ss = 0"
 proof -
-    have nforc:"~ k_mod.ready_force k ?msgs s" using nonForceAgain[of rho xi r k HO s ss] assms by auto
+    have nforc:"\<not> k_mod.ready_force k ?msgs s" using nonForceAgain[of rho xi r k HO s ss] assms by auto
     have nxt:"k_mod.SyncMod_nextState k xi s ?msgs ss" using transition[of rho r xi s ss k HO] assms by auto
-    hence "ALL q v. ?msgs q = Content (Val v) --> Suc v mod k >= x ss" using k_mod.SyncMod_nextState_def nforc by auto
+    hence "\<forall>q v. ?msgs q = Content (Val v) \<longrightarrow> Suc v mod k \<ge> x ss" using k_mod.SyncMod_nextState_def nforc by auto
     thus ?thesis using `?msgs p = Content (Val (k-1))` `k > 2` by fastforce
 qed
 
@@ -427,64 +427,64 @@ lemma A8 : assumes "k_mod.xi_nek HO xi"
 and run:"HORun (HOMachine_to_Algorithm (k_mod.SyncMod_HOMachine k)) rho HO" (is "HORun ?A _ _")
 and "k > 2"
 and "n > 4"
-and rd:"ALL p. round_force rho p < n - 4"
+and rd:"\<forall>p. round_force rho p < n - 4"
 and sxx:  "rho (n-3) xi = Active sxx"
 and sxs:  "rho (n-2) xi = Active sxs"
 and ss:   "rho (n-1) xi = Active ss"
 and sxiii:"rho n xi = Active sxiii"
 and sxii: "rho (Suc n) xi = Active sxii"
-and non_forc:"~ (EX sa saa. rho (round_force rho xi) xi = Active sa & (~ forc sa) & rho (Suc (round_force rho xi)) xi = Active saa & forc saa)"
+and non_forc:"\<not> (\<exists>sa saa. rho (round_force rho xi) xi = Active sa \<and> (\<not> forc sa) \<and> rho (Suc (round_force rho xi)) xi = Active saa \<and> forc saa)"
 and commS:"HOcommSchedule (k_mod.SyncMod_HOMachine k) (Schedule rho)"
 and "Suc (n-2) = n-1"
 and "Suc (n-3) = n-2"
 shows "x sxii = Suc (x sxiii) mod k"
 proof -
-    let ?msgx = "%p. HOrcvdMsgs ?A xi (HO (Suc (n-1)) xi) (rho (n-1)) p"
-    from rd have rd3:"ALL p. round_force rho p < n - 3"
+    let ?msgx = "\<lambda>p. HOrcvdMsgs ?A xi (HO (Suc (n-1)) xi) (rho (n-1)) p"
+    from rd have rd3:"\<forall>p. round_force rho p < n - 3"
         by (metis One_nat_def Suc_diff_Suc Suc_lessD add_Suc assms(4) numeral_3_eq_3 numeral_Bit0 one_add_one plus_1_eq_Suc trans_less_add2)
-    hence rd2:"ALL p. round_force rho p < n - 2"
+    hence rd2:"\<forall>p. round_force rho p < n - 2"
         by (metis One_nat_def Suc_diff_Suc Suc_lessD add_Suc assms(4) numeral_3_eq_3 numeral_Bit0 one_add_one plus_1_eq_Suc trans_less_add2)
-    hence rd1:"ALL p. round_force rho p < n - 1"
+    hence rd1:"\<forall>p. round_force rho p < n - 1"
         by (metis One_nat_def Suc_diff_Suc Suc_lessD add_Suc assms(4) numeral_Bit0 one_add_one plus_1_eq_Suc trans_less_add2)
-    hence rd0:"ALL p. round_force rho p < n"
+    hence rd0:"\<forall>p. round_force rho p < n"
         by (metis add_Suc add_diff_inverse_nat assms(4) not_less_eq numeral_Bit0 one_add_one trans_less_add2)
     have "k_mod.SyncMod_nextState k xi sxiii (HOrcvdMsgs ?A xi (HO (Suc n) xi) (rho n)) sxii"
         (is "k_mod.SyncMod_nextState k xi sxiii ?msgs sxii")
         using transition[of rho n xi sxiii sxii] run assms by auto
-    hence "~ k_mod.ready_force k ?msgs sxiii" using run nonForceAgain[of rho xi n k HO sxiii sxii] `k > 2` sxiii sxii rd0 by auto
-    hence "forc sxiii |
-        (EX p. ?msgs p = Content (Val (k-1))) |
-        (ALL p q v1 v2. ?msgs p = Content (Val v1) --> ?msgs q = Content (Val v2) --> v1 = v2)"
+    hence "\<not> k_mod.ready_force k ?msgs sxiii" using run nonForceAgain[of rho xi n k HO sxiii sxii] `k > 2` sxiii sxii rd0 by auto
+    hence "forc sxiii \<or>
+        (\<exists>p. ?msgs p = Content (Val (k-1))) \<or>
+        (\<forall>p q v1 v2. ?msgs p = Content (Val v1) \<longrightarrow> ?msgs q = Content (Val v2) \<longrightarrow> v1 = v2)"
         using k_mod.ready_force_def[of k ?msgs sxiii] by auto
     thus ?thesis
     proof
         assume "forc sxiii"
         thus ?thesis using neverForce[of rho xi k HO sxiii] run non_forc sxiii by auto
     next
-        assume "(EX p. ?msgs p = Content (Val (k-1))) |
-            (ALL p q v1 v2. ?msgs p = Content (Val v1) --> ?msgs q = Content (Val v2) --> v1 = v2)"
+        assume "(\<exists>p. ?msgs p = Content (Val (k-1))) \<or>
+            (\<forall>p q v1 v2. ?msgs p = Content (Val v1) \<longrightarrow> ?msgs q = Content (Val v2) \<longrightarrow> v1 = v2)"
         thus ?thesis 
         proof
-            assume "EX p. ?msgs p = Content (Val (k-1))"
+            assume "\<exists>p. ?msgs p = Content (Val (k-1))"
             then obtain p where "?msgs p = Content (Val (k-1))" by auto
             hence "x sxii = 0" using A7[of k rho HO n xi sxiii sxii p] assms sxii sxiii using rd0 by auto
             obtain sp spp where sp:"rho (n-1) p = Active sp" and spp:"rho n p = Active spp" and "x spp = k - 1"
                 using sending[of k rho HO xi "n-1" p "k-1"] assms `?msgs p = Content (Val (k-1))` by auto
-            hence "x spp <= Suc (x ss) mod k"
+            hence "x spp \<le> Suc (x ss) mod k"
                 using A5[of HO xi k rho "n-2" ss p sp spp] assms rd1 by auto
             hence "k-1 = Suc (x ss) mod k"
                 using `k > 2` `x spp = k-1` by (metis Suc_diff_1 le_less_Suc_eq less_Suc_eq_0_disj less_imp_Suc_add mod_less_divisor)
             moreover have "x ss < k" using transition assms ss by auto
             ultimately have "x ss = k - 2" using `k > 2`
                 by (metis Suc_lessI add_lessD1 diff_Suc_1 diff_diff_left less_numeral_extra(3) mod_less mod_self one_add_one zero_less_diff)
-            have "ALL q. ?msgx q ~= Content (Val (k-1))" 
+            have "\<forall>q. ?msgx q \<noteq> Content (Val (k-1))" 
             proof (rule+)
                 fix q
                 assume "?msgx q = Content (Val (k-1))"
                 (*hence "x sxiii = 0" using A7[of k rho HO "n-1" xi ss sxiii q] rd2 ss sxiii `k > 2` run by auto*)
                 then obtain sq sqq where sq:"rho (n-2) q = Active sq" and sqq:"rho (n-1) q = Active sqq" and "x sqq = k-1"
                     using sending[of k rho HO xi "n-2" q "k-1"] assms by auto
-                hence "x sqq <= Suc (x sxs) mod k"
+                hence "x sqq \<le> Suc (x sxs) mod k"
                     using assms A5[of HO xi k rho "n-3" sxs q sq sqq] sxs rd2 by auto
                 hence "k-1 = Suc (x sxs) mod k"
                     using `k > 2` `x sqq = k-1` by (metis Suc_diff_1 le_less_Suc_eq less_Suc_eq_0_disj less_imp_Suc_add mod_less_divisor)
@@ -492,65 +492,65 @@ proof -
                 moreover have "x sxs < k" using assms transition[of rho "n-3" xi sxx sxs k HO] sxs by auto
                 ultimately have "x sxs = k-2" by (smt Suc_1 Suc_inject assms(3) diff_Suc_Suc
                     less_imp_le_nat mod_Suc mod_if nat.simps(3) ordered_cancel_comm_monoid_diff_class.add_diff_assoc plus_1_eq_Suc)
-                let ?msg1 = "%p. HOrcvdMsgs ?A xi (HO (Suc (n-2)) xi) (rho (n-2)) p"
+                let ?msg1 = "\<lambda>p. HOrcvdMsgs ?A xi (HO (Suc (n-2)) xi) (rho (n-2)) p"
                 have nxt:"k_mod.SyncMod_nextState k xi sxs ?msg1 ss"
                     using transition[of rho "n-2" xi sxs ss k] assms by auto
-                have nfor:"~ k_mod.ready_force k ?msg1 sxs"
+                have nfor:"\<not> k_mod.ready_force k ?msg1 sxs"
                     using rd2 nonForceAgain[of rho xi "n-2" k HO sxs ss] assms by auto
-                hence "ALL qq. ?msg1 qq = Content (Val (k-1)) --> x ss <= Suc (k-1) mod k" using nxt by (simp add:k_mod.SyncMod_nextState_def)
-                hence "ALL qq. ?msg1 qq ~= Content (Val (k-1))" using `x ss = k-2` `k > 2` by auto
+                hence "\<forall>qq. ?msg1 qq = Content (Val (k-1)) \<longrightarrow> x ss \<le> Suc (k-1) mod k" using nxt by (simp add:k_mod.SyncMod_nextState_def)
+                hence "\<forall>qq. ?msg1 qq \<noteq> Content (Val (k-1))" using `x ss = k-2` `k > 2` by auto
 
                 have "?msg1 xi = Content (Val (k-2))" 
                     using sending_rec[of xi HO "n-2" xi k rho sxs] assms `x sxs = k-2`
                     by (metis `x sxs < k` k_mod.xi_nek_def)
                 then obtain qq v where "?msg1 qq = Content (Val v)" and "Suc v mod k = k-2" using `x ss = k - 2` nxt nfor k_mod.SyncMod_nextState_def by fastforce
-                have "EX ssqq sssqq. rho (n-3) qq = Active ssqq & rho (n-2) qq = Active sssqq & x sssqq = v"
+                have "\<exists>ssqq sssqq. rho (n-3) qq = Active ssqq \<and> rho (n-2) qq = Active sssqq \<and> x sssqq = v"
                     using sending[of k rho HO xi "n-3" qq v] `?msg1 qq = Content (Val v)` run `k > 2` assms(14) by simp
                 hence "v < k" using transition assms by auto
                 hence "?msg1 qq = Content (Val (k-3))" using `k > 2` `?msg1 qq = Content (Val v)` `Suc v mod k = k-2`
                     by (smt Suc_diff_Suc diff_Suc_1 diff_is_0_eq linorder_not_less mod_Suc mod_if numeral_3_eq_3 one_add_one plus_1_eq_Suc)
-                hence "EX p1 p2 v1 v2. ?msg1 p1 = Content (Val v1) & ?msg1 p2 = Content (Val v2) & v1 ~= v2" using `?msg1 xi = Content (Val (k-2))` `k > 2` by fastforce
-                hence "forc sxs" using nfor `ALL qq. ?msg1 qq ~= Content (Val (k-1))` k_mod.ready_force_def[of k ?msg1 sxs] `k > 2` by auto
+                hence "\<exists>p1 p2 v1 v2. ?msg1 p1 = Content (Val v1) \<and> ?msg1 p2 = Content (Val v2) \<and> v1 \<noteq> v2" using `?msg1 xi = Content (Val (k-2))` `k > 2` by fastforce
+                hence "forc sxs" using nfor `\<forall>qq. ?msg1 qq \<noteq> Content (Val (k-1))` k_mod.ready_force_def[of k ?msg1 sxs] `k > 2` by auto
                 thus "False" using neverForce[of rho xi k HO sxs] run non_forc sxs by auto
             qed
-            moreover have "~ k_mod.ready_force k ?msgx ss" using run nonForceAgain[of rho xi "n-1" k HO ss sxiii] `k > 2` ss sxiii rd1 by (simp add: nat_diff_split)
-            ultimately have "forc ss | (ALL p q v1 v2. ?msgx p = Content (Val v1) --> ?msgx q = Content (Val v2) --> v1 = v2)"
+            moreover have "\<not> k_mod.ready_force k ?msgx ss" using run nonForceAgain[of rho xi "n-1" k HO ss sxiii] `k > 2` ss sxiii rd1 by (simp add: nat_diff_split)
+            ultimately have "forc ss \<or> (\<forall>p q v1 v2. ?msgx p = Content (Val v1) \<longrightarrow> ?msgx q = Content (Val v2) \<longrightarrow> v1 = v2)"
                 using k_mod.ready_force_def[of k ?msgx ss] by auto
             thus ?thesis
             proof
                 assume "forc ss"
                 thus ?thesis using neverForce[of rho xi k HO ss] run non_forc ss by auto
             next
-                assume "ALL p q v1 v2. ?msgx p = Content (Val v1) --> ?msgx q = Content (Val v2) --> v1 = v2"
+                assume "\<forall>p q v1 v2. ?msgx p = Content (Val v1) \<longrightarrow> ?msgx q = Content (Val v2) \<longrightarrow> v1 = v2"
                 moreover have "?msgx xi = Content (Val (k-2))"
                     using ` x ss = k - 2` sending_rec[of xi HO "n-1" xi k rho ss] `k_mod.xi_nek HO xi` `k > 2` ss `n > 4`
                     by (simp add: k_mod.xi_nek_def run less_natE)
-                ultimately have "ALL p v. ?msgx p = Content (Val v) --> v = k - 2" by auto
+                ultimately have "\<forall>p v. ?msgx p = Content (Val v) \<longrightarrow> v = k - 2" by auto
                 have "k_mod.SyncMod_nextState k xi ss ?msgx sxiii"
                     using transition[of rho "n-1" xi ss sxiii k] assms by auto
-                hence "EX q v. ?msgx q = Content (Val v) & Suc v mod k = x sxiii"
+                hence "\<exists>q v. ?msgx q = Content (Val v) \<and> Suc v mod k = x sxiii"
                   using `?msgx xi = Content (Val (k-2))` `~ k_mod.ready_force k ?msgx ss`
                   unfolding k_mod.SyncMod_nextState_def by fastforce
-                hence "EX v. v = k - 2 & Suc v mod k = x sxiii" using `ALL p v. ?msgx p = Content (Val v) --> v = k - 2` by auto
+                hence "\<exists>v. v = k - 2 \<and> Suc v mod k = x sxiii" using `\<forall>p v. ?msgx p = Content (Val v) \<longrightarrow> v = k - 2` by auto
                 hence "x sxiii = k - 1" using `k > 2` by fastforce
                 thus ?thesis using `x sxii = 0` `k > 2` by auto
             qed
         next
-            assume "ALL p q v1 v2. ?msgs p = Content (Val v1) --> ?msgs q = Content (Val v2) --> v1 = v2"
+            assume "\<forall>p q v1 v2. ?msgs p = Content (Val v1) \<longrightarrow> ?msgs q = Content (Val v2) \<longrightarrow> v1 = v2"
             moreover have "x sxiii < k" 
                 using transition[of rho "n-1" xi ss sxiii k] assms by auto
             hence "?msgs xi = Content (Val (x sxiii))"
                 using sending_rec[of xi HO n xi k rho sxiii] `k_mod.xi_nek HO xi` `k > 2` sxiii `n > 4`
                 by (simp add: k_mod.xi_nek_def run less_natE)
-            ultimately have "ALL p v. ?msgs p = Content (Val v) --> v = x sxiii" by auto
+            ultimately have "\<forall>p v. ?msgs p = Content (Val v) \<longrightarrow> v = x sxiii" by auto
             have "k_mod.SyncMod_nextState k xi sxiii ?msgs sxii"
                 using transition[of rho n xi sxiii sxii k] assms by auto
-            moreover have "~ k_mod.ready_force k ?msgs sxiii"
+            moreover have "\<not> k_mod.ready_force k ?msgs sxiii"
                 using run nonForceAgain[of rho xi n k HO sxiii sxii] `k > 2` sxii sxiii rd0 by simp 
-            ultimately have "EX q v. ?msgs q = Content (Val v) & Suc v mod k = x sxii"
+            ultimately have "\<exists>q v. ?msgs q = Content (Val v) \<and> Suc v mod k = x sxii"
               using `?msgs xi = Content (Val (x sxiii))`
               unfolding k_mod.SyncMod_nextState_def by fastforce
-            hence "EX v. v = x sxiii & Suc v mod k = x sxii" using `ALL p v. ?msgs p = Content (Val v) --> v = x sxiii` by auto
+            hence "\<exists>v. v = x sxiii \<and> Suc v mod k = x sxii" using `\<forall>p v. ?msgs p = Content (Val v) \<longrightarrow> v = x sxiii` by auto
             thus ?thesis by auto
         qed
     qed
@@ -562,51 +562,51 @@ and "k > 2"
 assumes commS:"HOcommSchedule (k_mod.SyncMod_HOMachine k) (Schedule rho)"
 shows "k_mod.safety k rho"
 proof -
-    have monov:"ALL p r s ss. rho r p = Active s --> rho (Suc r) p = Active ss --> fire ss --> ~ fire s --> monovalent rho 0 r & rho r xi ~= Asleep"
+    have monov:"\<forall>p r s ss. rho r p = Active s \<longrightarrow> rho (Suc r) p = Active ss \<longrightarrow> fire ss \<longrightarrow> \<not> fire s \<longrightarrow> monovalent rho 0 r \<and> rho r xi \<noteq> Asleep"
     proof (rule+)
         fix p r s ss
-        assume s:"rho r p = Active s" and ss:"rho (Suc r) p = Active ss" and "fire ss" and "~ fire s" 
-        show "monovalent rho 0 r" and "rho r xi ~= Asleep"
+        assume s:"rho r p = Active s" and ss:"rho (Suc r) p = Active ss" and "fire ss" and "\<not> fire s" 
+        show "monovalent rho 0 r" and "rho r xi \<noteq> Asleep"
         proof -
-            let ?msgs = "%q. HOrcvdMsgs ?A p (HO (Suc r) p) (rho r) q"
+            let ?msgs = "\<lambda>q. HOrcvdMsgs ?A p (HO (Suc r) p) (rho r) q"
             have "k_mod.SyncMod_nextState k p s ?msgs ss"
                 using transition[of rho r p s ss k] assms s ss by auto
             hence "k_mod.ready_fire k ?msgs" using k_mod.SyncMod_nextState_def `fire ss` `~ fire s` by auto
             hence "?msgs xi = Content (Val (k-1))" using k_mod.xi_nek_def `k_mod.xi_nek HO xi` k_mod.ready_fire_def HOrcvdMsgs_def
                 by (metis HOrcvMsgs_q.elims message.distinct(3) message.distinct(5))
-            hence "rho r xi ~= Asleep" using HOrcvdMsgs_def[of ?A p "HO (Suc r) p" "rho r"] assms by auto
-            have "r ~= 0"
+            hence "rho r xi \<noteq> Asleep" using HOrcvdMsgs_def[of ?A p "HO (Suc r) p" "rho r"] assms by auto
+            have "r \<noteq> 0"
             proof
                 assume "r = 0"
-                then obtain sz where sz:"rho 0 xi = Active sz" using `rho r xi ~= Asleep` by (cases "rho 0 xi") auto
-                hence "?msgs xi = (if xi : HO (Suc 0) p then Content Nope else Void)"
+                then obtain sz where sz:"rho 0 xi = Active sz" using `rho r xi \<noteq> Asleep` by (cases "rho 0 xi") auto
+                hence "?msgs xi = (if xi \<in> HO (Suc 0) p then Content Nope else Void)"
                   using starting[of 0 rho xi k HO sz] s assms `r = 0` by auto
                 thus "False" using `?msgs xi = Content (Val (k-1))` by auto
             qed
             then obtain sx sxx where "rho (r-1) xi = Active sx" and "rho r xi = Active sxx" and "x sxx = k-1"
                 using `?msgs xi = Content (Val (k-1))` sending[of k rho HO p "r-1" xi "k-1"] run by auto
-            thus "monovalent rho 0 r" and "rho r xi ~= Asleep" using A2[of HO xi k rho r sxx] assms by auto
+            thus "monovalent rho 0 r" and "rho r xi \<noteq> Asleep" using A2[of HO xi k rho r sxx] assms by auto
         qed
     qed
     show ?thesis
-    proof (cases "EX p r s ss. rho r p = Active s & rho (Suc r) p = Active ss & fire ss & ~ fire s")
+    proof (cases "\<exists>p r s ss. rho r p = Active s \<and> rho (Suc r) p = Active ss \<and> fire ss \<and> \<not> fire s")
         case False
-        hence "ALL p rf ss sf. rho rf p = Active ss -->
-                    (~ fire ss) --> rho (Suc rf) p = Active sf --> fire sf --> rf mod k = 0" by blast
-        hence "EX c. ALL p rf ss sf. rho rf p = Active ss -->
-                    (~ fire ss) --> rho (Suc rf) p = Active sf --> fire sf --> rf mod k = c" by auto
+        hence "\<forall>p rf ss sf. rho rf p = Active ss \<longrightarrow>
+                    (\<not> fire ss) \<longrightarrow> rho (Suc rf) p = Active sf \<longrightarrow> fire sf \<longrightarrow> rf mod k = 0" by blast
+        hence "\<exists>c. \<forall>p rf ss sf. rho rf p = Active ss \<longrightarrow>
+                    (\<not> fire ss) \<longrightarrow> rho (Suc rf) p = Active sf \<longrightarrow> fire sf \<longrightarrow> rf mod k = c" by auto
         thus ?thesis by (simp add:k_mod.safety_def)
     next
         case True
-        then obtain p r s ss where s:"rho r p = Active s" and ss:"rho (Suc r) p = Active ss" and "fire ss" and "~ fire s" by auto
-        hence "monovalent rho 0 r" and "rho r xi ~= Asleep" using monov by auto
+        then obtain p r s ss where s:"rho r p = Active s" and ss:"rho (Suc r) p = Active ss" and "fire ss" and "\<not> fire s" by auto
+        hence "monovalent rho 0 r" and "rho r xi \<noteq> Asleep" using monov by auto
         then obtain sx where "rho r xi = Active sx" by (cases "rho r xi") auto
-        have "ALL p rf ss sf. rho rf p = Active ss -->
-                    (~ fire ss) --> rho (Suc rf) p = Active sf --> fire sf --> rf mod k = r mod k"
+        have "\<forall>p rf ss sf. rho rf p = Active ss \<longrightarrow>
+                    (\<not> fire ss) \<longrightarrow> rho (Suc rf) p = Active sf \<longrightarrow> fire sf \<longrightarrow> rf mod k = r mod k"
         proof (rule+)
             fix q rq sq sqq
-            assume sq:"rho rq q = Active sq" and sqq:"rho (Suc rq) q = Active sqq" and "~ fire sq" and "fire sqq"
-            hence "monovalent rho 0 rq" and "rho rq xi ~= Asleep" using monov by auto
+            assume sq:"rho rq q = Active sq" and sqq:"rho (Suc rq) q = Active sqq" and "\<not> fire sq" and "fire sqq"
+            hence "monovalent rho 0 rq" and "rho rq xi \<noteq> Asleep" using monov by auto
             then obtain sxq where "rho rq xi = Active sxq" by (cases "rho rq xi") auto
             show "rq mod k = r mod k" 
             proof (cases "rq > r")
@@ -623,8 +623,8 @@ proof -
                 ultimately show ?thesis by (metis False less_numeral_extra(3) linorder_not_less mod_eq_dvd_iff_nat mod_greater_zero_iff_not_dvd)
             qed
         qed
-        hence "EX c. ALL p rf ss sf. rho rf p = Active ss -->
-                    (~ fire ss) --> rho (Suc rf) p = Active sf --> fire sf --> rf mod k = c" by auto
+        hence "\<exists>c. \<forall>p rf ss sf. rho rf p = Active ss \<longrightarrow>
+                    (\<not> fire ss) \<longrightarrow> rho (Suc rf) p = Active sf \<longrightarrow> fire sf \<longrightarrow> rf mod k = c" by auto
         thus ?thesis using k_mod.safety_def by auto
     qed
 qed
@@ -638,9 +638,9 @@ shows "k_mod.liveness rho"
 proof -
     let ?txi = "round_force rho xi"
     show ?thesis
-    proof (cases "EX sa saa. rho ?txi xi = Active sa & (~ forc sa) & rho (Suc ?txi) xi = Active saa & forc saa")
+    proof (cases "\<exists>sa saa. rho ?txi xi = Active sa \<and> (\<not> forc sa) \<and> rho (Suc ?txi) xi = Active saa \<and> forc saa")
         case True
-        then obtain sx sxx where "rho ?txi xi = Active sx" and "~ forc sx" and "rho (Suc ?txi) xi = Active sxx" and "forc sxx" by auto
+        then obtain sx sxx where "rho ?txi xi = Active sx" and "\<not> forc sx" and "rho (Suc ?txi) xi = Active sxx" and "forc sxx" by auto
         hence nxt:"k_mod.SyncMod_nextState k xi sx (HOrcvdMsgs ?A xi (HO (Suc ?txi) xi) (rho ?txi)) sxx" (is "SyncMod.k_mod.SyncMod_nextState k xi sx ?msgs sxx")
             using transition[of rho ?txi xi sx sxx k HO] assms by auto
         hence "k_mod.ready_force k ?msgs sx" using k_mod.SyncMod_nextState_def `~ forc sx` `forc sxx` by auto
@@ -648,51 +648,51 @@ proof -
         thus ?thesis using A4 `rho (Suc ?txi) xi = Active sxx` assms by auto
     next
         case False
-        have "EX n. Schedule rho n = UNIV" using commS by (simp add:k_mod.SyncMod_HOMachine_def k_mod.SyncMod_commSchedule_def )
-        then obtain n :: nat where "ALL p. rho n p ~= Asleep" unfolding Schedule_def by auto
+        have "\<exists>n. Schedule rho n = UNIV" using commS by (simp add:k_mod.SyncMod_HOMachine_def k_mod.SyncMod_commSchedule_def )
+        then obtain n :: nat where "\<forall>p. rho n p \<noteq> Asleep" unfolding Schedule_def by auto
         let ?n = "Suc (Suc (Suc (Suc (Suc n)))) + Sum ( (round_force rho) ` UNIV)"
         obtain sxi where "rho ?n xi = Active sxi" 
-            using nonAsleepAgain[of rho n xi _ _ _ "Suc (Suc (Suc (Suc (Suc (Sum ( (round_force rho) ` UNIV))))))"] run HORun_def `ALL p. rho n p ~= Asleep`
+            using nonAsleepAgain[of rho n xi _ _ _ "Suc (Suc (Suc (Suc (Suc (Sum ( (round_force rho) ` UNIV))))))"] run HORun_def `\<forall>p. rho n p \<noteq> Asleep`
             by (smt add.commute add_Suc_shift)
         show ?thesis
-        proof (cases "EX v :: nat. v < k & monovalent rho v ?n")
+        proof (cases "\<exists>v :: nat. v < k \<and> monovalent rho v ?n")
             case True
             thus ?thesis using A6[of HO xi k rho ?n sxi] assms `rho ?n xi = Active sxi` by (metis mod_if)
         next
             case False
-            have escalier:"ALL i sxii. rho (?n + i) xi = Active sxii --> x sxii = (x sxi + i) mod k"
+            have escalier:"\<forall>i sxii. rho (?n + i) xi = Active sxii \<longrightarrow> x sxii = (x sxi + i) mod k"
             proof (rule allI)+
                 fix i sxii
-                show "rho (?n + i) xi = Active sxii --> x sxii = (x sxi + i) mod k"
+                show "rho (?n + i) xi = Active sxii \<longrightarrow> x sxii = (x sxi + i) mod k"
                 proof (induction i arbitrary:sxii)
                     case 0
                     obtain sx where "rho (?n-1) xi = Active sx"
-                        using nonAsleepAgain[of rho n xi _ _ _ "Suc (Suc (Suc (Suc (Sum ( (round_force rho) ` UNIV)))))"] run HORun_def `ALL p. rho n p ~= Asleep`
+                        using nonAsleepAgain[of rho n xi _ _ _ "Suc (Suc (Suc (Suc (Sum ( (round_force rho) ` UNIV)))))"] run HORun_def `\<forall>p. rho n p \<noteq> Asleep`
                         by (smt Nat.add_diff_assoc2 add.commute diff_Suc_1 le_add1 plus_1_eq_Suc)
                     hence "x sxi < k" using transition[of rho "?n-1" xi sx sxi] run `rho ?n xi = Active sxi` assms(3) by auto
-                    thus "rho (?n + 0) xi = Active sxii --> x sxii = (x sxi + 0) mod k" using `rho ?n xi = Active sxi` by auto
+                    thus "rho (?n + 0) xi = Active sxii \<longrightarrow> x sxii = (x sxi + 0) mod k" using `rho ?n xi = Active sxi` by auto
                 next
                     case (Suc ii)
-                    show "rho (?n + Suc ii) xi = Active sxii --> x sxii = (x sxi + Suc ii) mod k"
+                    show "rho (?n + Suc ii) xi = Active sxii \<longrightarrow> x sxii = (x sxi + Suc ii) mod k"
                     proof 
                         assume "rho (?n + Suc ii) xi = Active sxii"
                         hence "rho (Suc ?n + ii) xi = Active sxii" by auto
-                        moreover have "ALL p. round_force rho p < ?n +ii - 4"
+                        moreover have "\<forall>p. round_force rho p < ?n +ii - 4"
                         proof
                             fix p
-                            have rd_forc:"round_force rho p <= Sum ((round_force rho) ` UNIV)"
+                            have rd_forc:"round_force rho p \<le> Sum ((round_force rho) ` UNIV)"
                                 by (meson finite_UNIV finite_imageI le0 range_eqI sum_nonneg_leq_bound)
-                            hence "round_force rho p <= Sum ((round_force rho) ` UNIV) + ((Suc (Suc (Suc (Suc n)))) + ii - 4)" using trans_le_add1 by blast
-                            moreover have "Suc (Suc (Suc (Suc n))) + ii >= 4" by auto
+                            hence "round_force rho p \<le> Sum ((round_force rho) ` UNIV) + ((Suc (Suc (Suc (Suc n)))) + ii - 4)" using trans_le_add1 by blast
+                            moreover have "Suc (Suc (Suc (Suc n))) + ii \<ge> 4" by auto
                             hence " Sum ((round_force rho) ` UNIV) + ((Suc (Suc (Suc (Suc n)))) + ii - 4) =
                                     Sum ((round_force rho) ` UNIV) + (Suc (Suc (Suc (Suc n)))) + ii - 4"
                                 using add_diff_assoc[of 4 "Suc (Suc (Suc (Suc n))) + ii" "Sum (range (round_force rho))"] by fastforce
-                            ultimately have "round_force rho p <= Sum ((round_force rho) ` UNIV) + (Suc (Suc (Suc (Suc n)))) + ii - 4"
+                            ultimately have "round_force rho p \<le> Sum ((round_force rho) ` UNIV) + (Suc (Suc (Suc (Suc n)))) + ii - 4"
                                 by fastforce
                             thus "round_force rho p < ?n + ii - 4" by auto
                         qed
                         moreover obtain sxx where "rho (n+Suc (Suc (Sum ( (round_force rho) ` UNIV)))+ii) xi = Active sxx"
-                            using nonAsleepAgain[of rho n xi _ _ _ "Suc (Suc (Sum ((round_force rho) ` UNIV)))+ii"] run HORun_def `ALL p. rho n p ~= Asleep`
+                            using nonAsleepAgain[of rho n xi _ _ _ "Suc (Suc (Sum ((round_force rho) ` UNIV)))+ii"] run HORun_def `\<forall>p. rho n p \<noteq> Asleep`
                             by (metis add.assoc)
                         hence "rho (?n+ii-3) xi = Active sxx" by fastforce
                         moreover from this obtain sxs where "rho (?n+ii-2) xi = Active sxs"
@@ -707,22 +707,22 @@ proof -
                         moreover have "?n+ii > 4" by auto
                         ultimately have "x sxii = Suc (x sxiii) mod k"
                             using A8[of HO xi k rho "?n+ii" sxx sxs ss sxiii sxii] assms
-                            `~ (EX sa saa. rho ?txi xi = Active sa & (~ forc sa) & rho (Suc ?txi) xi = Active saa & forc saa)` by fastforce
+                            `~ (\<exists>sa saa. rho ?txi xi = Active sa \<and> (~ forc sa) \<and> rho (Suc ?txi) xi = Active saa \<and> forc saa)` by fastforce
                         thus "x sxii = (x sxi + Suc ii) mod k" using Suc.IH[of sxiii] `rho (?n+ii) xi = Active sxiii` by presburger
                     qed
                 qed
             qed
             obtain sxx where "rho (?n-1) xi = Active sxx" 
                 using nonAsleepAgain[of rho n xi _ _ _ "Suc (Suc (Suc (Suc (Suc (Sum (range (round_force rho)))))))-1"]
-                run HORun_def add_diff_assoc[of 1 "Suc (Suc (Suc (Suc (Suc (Sum (range (round_force rho)))))))" n] `ALL p. rho n p ~= Asleep`
+                run HORun_def add_diff_assoc[of 1 "Suc (Suc (Suc (Suc (Suc (Sum (range (round_force rho)))))))" n] `\<forall>p. rho n p \<noteq> Asleep`
                 by (smt add_Suc add_Suc_shift diff_Suc_1)
-            hence "k-1 >= x sxi"
+            hence "k-1 \<ge> x sxi"
                 using transition[of rho "?n-1" xi sxx sxi k] assms `rho ?n xi = Active sxi` by fastforce
             obtain s where "rho (?n+(k-1-x sxi)) xi = Active s"
                 using nonAsleepAgain[of rho ?n xi _ _ _ "k-1-x sxi"] run HORun_def `rho ?n xi = Active sxi` by fastforce
 
             hence "x s = (x sxi + (k-1-x sxi)) mod k" using escalier by auto
-            hence "x s = k - 1" using `k - 1 >= x sxi` by (simp add: add_diff_inverse_nat nat_diff_split)
+            hence "x s = k - 1" using `k - 1 \<ge> x sxi` by (simp add: add_diff_inverse_nat nat_diff_split)
             thus ?thesis using A4[of HO xi k rho "?n+(k-1-x sxi)" s] assms `rho (?n+(k-1-x sxi)) xi = Active s` by auto
         qed
     qed
