proof_Isabelle/sync-mod/Views.thy
@@ -12,16 +12,16 @@ datatype tree_2col =
 
 fun list_in where
 "list_in v [] = False" |
-"list_in v (a#l) = ((v = a) | list_in v l)"
+"list_in v (a#l) = ((v = a) \<or> list_in v l)"
 
 definition view_compute where
-"view_compute = (| 
-    CinitState = (%p st _. st = Initial),
-    sendMsg = (%_ _ st. st),
+"view_compute = \<lparr> 
+    CinitState = (\<lambda>p st _. st = Initial),
+    sendMsg = (\<lambda>_ _ st. st),
     CnextState = (%_ s msgs _ s'. s' = Node
-        (EX p. msgs p = Bot)
-        (SOME l :: tree_2col list. ALL child :: tree_2col. ((list_in child l) = (EX p. msgs p = Content child))))
-|)"
+        (\<exists>p. msgs p = Bot)
+        (SOME l :: tree_2col list. \<forall>child :: tree_2col. ((list_in child l) = (\<exists>p. msgs p = Content child))))
+\<rparr>"
 
 record locState = 
      x :: nat
@@ -31,59 +31,59 @@ record locState =
      level :: nat
 
 fun tree_to_state where
-"tree_to_state k Initial = (| x = 0, conc = False, ready = False, forc = 0, level = 0 |)" |
+"tree_to_state k Initial = \<lparr> x = 0, conc = False, ready = False, forc = 0, level = 0 \<rparr>" |
 "tree_to_state k (Node passiv_rcvd siblings) = (
     let msgs = List.map (tree_to_state k) siblings in
     let max_f = Max (forc ` (List.set msgs)) in
-    let v = Suc (LEAST v. EX s. list_in s msgs & x s = v) in 
-    let concr = ~ passiv_rcvd & (ALL s. list_in s msgs --> conc s) in
-    let readyr = ALL s. list_in s msgs --> ready s in
-    (| x = v, conc = concr | v mod k = 0, ready = readyr | v mod k = 0, forc = 0, level = 0 |))"
+    let v = Suc (LEAST v. \<exists>s. list_in s msgs \<and> x s = v) in 
+    let concr = \<not> passiv_rcvd \<and> (\<forall>s. list_in s msgs \<longrightarrow> conc s) in
+    let readyr = \<forall>s. list_in s msgs \<longrightarrow> ready s in
+    \<lparr> x = v, conc = concr \<or> v mod k = 0, ready = readyr \<or> v mod k = 0, forc = 0, level = 0 \<rparr>)"
 
 definition view where
 "view rho HO p t 0 = Initial" |
-"view rho HO p t (Suc r) = (UN q : incoming rho HO p t r. if rho (t-r) q = Asleep then {q} else HO (t-r) q)"
+"view rho HO p t (Suc r) = (UN q \<in> incoming rho HO p t r. if rho (t-r) q = Asleep then {q} else HO (t-r) q)"
 
 
 definition set_computable  where
-"set_computable f == EX algo comput. ALL rho HO r p s. HORun algo rho HO --> rho r p = Active s --> f rho HO p r = comput s"
+"set_computable f \<equiv> \<exists>algo comput. \<forall>rho HO r p s. HORun algo rho HO \<longrightarrow> rho r p = Active s \<longrightarrow> f rho HO p r = comput s"
 
 fun incoming where
 "incoming rho HO p t 0 = {p}" |
-"incoming rho HO p t (Suc r) = (UN q : incoming rho HO p t r. if rho (t-r) q = Asleep then {q} else HO (t-r) q)"
+"incoming rho HO p t (Suc r) = (UN q \<in> incoming rho HO p t r. if rho (t-r) q = Asleep then {q} else HO (t-r) q)"
 
 definition incoming_compute where
-"incoming_compute = (| 
-    CinitState = (%p st _. st = {p}),
-    sendMsg = (%_ _ st. st),
-    CnextState = (%_ s msgs _ s'. s' = Union (range (%p.
+"incoming_compute = \<lparr> 
+    CinitState = (\<lambda>p st _. st = {p}),
+    sendMsg = (\<lambda>_ _ st. st),
+    CnextState = (%_ s msgs _ s'. s' = Union (range (\<lambda>p.
         if msgs p = Void then {} else
         if msgs p = Bot then {p} else
             SOME s. msgs p = Content s)))
-|)"
+\<rparr>"
 
 lemma incoming_computable : 
 assumes run:"HORun incoming_compute rho HO"
-shows "ALL r t p. (r = 0 | rho (r-1) p = Asleep) --> rho r p ~= Asleep --> (SOME s. rho (r+t) p = Active s) = incoming rho HO p r t"
+shows "\<forall>r t p. (r = 0 \<or> rho (r-1) p = Asleep) \<longrightarrow> rho r p \<noteq> Asleep \<longrightarrow> (SOME s. rho (r+t) p = Active s) = incoming rho HO p r t"
 proof 
     fix r 
-    show "ALL t p. (r = 0 | rho (r-1) p = Asleep) --> rho r p ~= Asleep --> (SOME s. rho (r+t) p = Active s) = incoming rho HO p r t"
+    show "\<forall>t p. (r = 0 \<or> rho (r-1) p = Asleep) \<longrightarrow> rho r p \<noteq> Asleep \<longrightarrow> (SOME s. rho (r+t) p = Active s) = incoming rho HO p r t"
     proof
         fix t
-        show "ALL p. (r = 0 | rho (r-1) p = Asleep) --> rho r p ~= Asleep --> (SOME s. rho (r+t) p = Active s) = incoming rho HO p r t"
+        show "\<forall>p. (r = 0 \<or> rho (r-1) p = Asleep) \<longrightarrow> rho r p \<noteq> Asleep \<longrightarrow> (SOME s. rho (r+t) p = Active s) = incoming rho HO p r t"
 proof (induction "r+t")
     case 0
     show ?case
     proof (rule allI impI)+
         fix p
-        assume "r = 0 | rho (r-1) p = Asleep"
-        assume act:"rho r p ~= Asleep"
+        assume "r = 0 \<or> rho (r-1) p = Asleep"
+        assume act:"rho r p \<noteq> Asleep"
         from this "0.hyps" obtain s where s:"rho 0 p = Active s" using the_state.cases by auto 
-        from run have "CHOinitConfig incoming_compute rho (%_ _. undefined)" (is "CHOinitConfig ?A _ _")
+        from run have "CHOinitConfig incoming_compute rho (\<lambda>_ _. undefined)" (is "CHOinitConfig ?A _ _")
             by (simp add: HORun_def CHORun_def)
         moreover from act "0.hyps" have "first_awake rho p = 0"
             unfolding first_awake_def by auto
-        moreover from act have "~ always_asleep rho p" unfolding always_asleep_def by auto
+        moreover from act have "\<not> always_asleep rho p" unfolding always_asleep_def by auto
         ultimately have "CinitState incoming_compute p s undefined" using assms s unfolding CHOinitConfig_def by auto
         hence "s = {p}" unfolding incoming_compute_def by auto
         thus "(SOME s. rho (r+t) p = Active s) = incoming rho HO p r t" using "0.hyps" by (simp add:s)
@@ -93,7 +93,7 @@ next
     show ?case
     proof (rule allI impI)+
         fix p
-        assume "r = 0 | rho (r-1) p = Asleep"
-        assume act:"rho r p ~= Asleep"
+        assume "r = 0 \<or> rho (r-1) p = Asleep"
+        assume act:"rho r p \<noteq> Asleep"
         from nonAsleepAgain[of _ r p] run this obtain s where "rho (r+t) p = Active s" unfolding HORun_def by blast
 
