proof_Isabelle/otr/Tiroir.thy
@@ -2,16 +2,16 @@ theory Tiroir
   imports Main
 begin
 
-lemma tiroir: assumes fini:"finite {v. E v}" shows "finite {f v | v. E v}"
+lemma tiroir: assumes fini:"finite {v. E v}" shows "finite {f v \<or> v. E v}"
 proof -
   from assms have "finite (f ` {v. E v})" .. (* finite_imageI *)
   thus ?thesis by (simp add: setcompr_eq_image) 
 qed
 
 lemma tiroir2: assumes inject:"\<forall>v1 v2. f v1 = f v2 \<longrightarrow> v1 = v2"
-  shows "finite {f v | v. E v} \<longrightarrow> finite {v. E v}"
+  shows "finite {f v \<or> v. E v} \<longrightarrow> finite {v. E v}"
 proof
-  assume "finite {f v | v. E v}"
+  assume "finite {f v \<or> v. E v}"
   hence "finite (f ` {v . E v})" by (simp add: image_Collect) 
   moreover
   from inject have "inj_on f {v . E v}" by (simp add: inj_onI) 
